Coq/src/Step.v
@@ -5,10 +5,11 @@ Require Import AuxDef.
 Require Import EventStructure.
 Require Import Consistency.
 Require Import BasicStep.
+Require Import AddJF.
+Require Import AddEW.
+Require Import AddCO.
 
 Set Implicit Arguments.
-
-Module ESstep.
 
 Notation "'E' S" := S.(ES.acts_set) (at level 10).
 Notation "'Einit' S"  := S.(ES.acts_init_set) (at level 10).
@@ -50,9 +51,9 @@ Notation "'Acq' S" := (fun a => is_true (is_acq S.(ES.lab) a)) (at level 10).
 Notation "'Acqrel' S" := (fun a => is_true (is_acqrel S.(ES.lab) a)) (at level 10).
 Notation "'Sc' S" := (fun a => is_true (is_sc S.(ES.lab) a)) (at level 10).
 
-Notation "'same_mod' S" := (same_mod S.(ES.lab)) (at level 10).
-Notation "'same_loc' S" := (same_loc S.(ES.lab)) (at level 10).
-Notation "'same_val' S" := (same_val S.(ES.lab)) (at level 10).
+(* Notation "'same_mod' S" := (same_mod S.(ES.lab)) (at level 10). *)
+(* Notation "'same_loc' S" := (same_loc S.(ES.lab)) (at level 10). *)
+(* Notation "'same_val' S" := (same_val S.(ES.lab)) (at level 10). *)
 
 Notation "'K' S" := (S.(ES.cont_set)) (at level 10).
 
@@ -61,1557 +62,255 @@ Notation "'Mod_' S" := (fun m x => mod S x = m) (at level 9).
 Notation "'Loc_' S" := (fun l x => loc S x = l) (at level 9).
 Notation "'Val_' S" := (fun v e => val S e = v) (at level 9).
 
-Definition jf_delta w r : relation eventid := 
-  singl_rel w r.
-
-Hint Unfold jf_delta : ESStepDb.
-
-Definition add_jf w r' S S' : Prop :=  
-  ⟪ rE' : E S' r' ⟫ /\
-  ⟪ rR' : R S' r' ⟫ /\
-  ⟪ wE : E S w ⟫ /\
-  ⟪ wW : W S w ⟫ /\
-  ⟪ LOC : same_loc S' w r' ⟫ /\
-  ⟪ VAL : same_val S' w r' ⟫ /\
-  ⟪ nCF : ~ cf S' w r' ⟫ /\
-  ⟪ JF' : jf S' ≡ jf S ∪ jf_delta w r' ⟫.
-
-Definition ew_delta ws w : relation eventid := 
-  eq w × eq w ∪ (ws × eq w)^⋈.
-
-Hint Unfold ew_delta : ESStepDb.
-
-Definition add_ew ews w' S S' : Prop :=   
-  ⟪ wE' : E S' w' ⟫ /\
-  ⟪ wW' : W S' w' ⟫ /\
-  ⟪ ewsE : ews ⊆₁ E S ⟫ /\
-  ⟪ ewsW : ews ⊆₁ W S ⟫ /\
-  ⟪ ewsRLX : ews ⊆₁ Rlx S ⟫ /\
-  ⟪ ewsMOD : ews ⊆₁ same_mod S' w' ⟫ /\
-  ⟪ ewsLOC : ews ⊆₁ same_loc S' w' ⟫ /\
-  ⟪ ewsVAL : ews ⊆₁ same_val S' w' ⟫ /\
-  ⟪ ewsCF : ews ⊆₁ cf S' w' ⟫ /\
-  ⟪ ewsEW : ews × ews ⊆ ew S ⟫ /\
-  ⟪ ewsEWprcl : dom_rel (ew S ⨾ ⦗ews⦘) ⊆₁ ews ⟫ /\
-  ⟪ EW' : ew S' ≡ ew S ∪ ew_delta ews w' ⟫. 
-
-Definition ws_compl ews ws S := 
-  codom_rel (⦗ews ∪₁ ws⦘ ⨾ co S) \₁ (ews ∪₁ ws).
-
-Definition co_delta ews ws w' S : relation eventid := 
-  ws × eq w' ∪ eq w' × ws_compl ews ws S.
-
-Hint Unfold ws_compl co_delta : ESStepDb.
-
-Definition add_co ews ws w' S S' : Prop := 
-  ⟪ wE' : E S' w' ⟫ /\
-  ⟪ wW' : W S' w' ⟫ /\
-  ⟪ wsE : ws ⊆₁ E S ⟫ /\
-  ⟪ wsW : ws ⊆₁ W S ⟫ /\
-  ⟪ wsLOC : ws ⊆₁ same_loc S' w' ⟫ /\
-  ⟪ ws_ews : ws ∩₁ ews ⊆₁ ∅ ⟫ /\
-  ⟪ wsEinit : (Einit S ∩₁ Loc_ S (loc S' w')) ⊆₁ ws ⟫ /\
-  ⟪ wsCOEWprcl : dom_rel ((co S)^? ⨾ (ew S)^? ⨾ ⦗ws⦘) ⊆₁ ws ⟫ /\
-  ⟪ ewsCOprcl : dom_rel (co S ⨾ ⦗ews⦘) ⊆₁ ws ⟫ /\
-  ⟪ ewsCOprcl : dom_rel (co S ⨾ ⦗ews⦘) ⊆₁ ws ⟫ /\
-  (* ⟪ wsNCF : ws ⊆₁ dom_rel ((co S)^? ⨾ (ew S)^? ⨾ ⦗set_compl (cf S' w')⦘) ⟫ /\ *)
-  ⟪ CO' : co S' ≡ co S ∪ co_delta ews ws w' S ⟫.
-
-Definition t_fence
+Definition fence_step
            (e  : eventid)
            (e' : option eventid)
            (S S' : ES.t) : Prop :=
-  ⟪ ENONE : e' = None ⟫ /\
+  ⟪ nUPD : e' = None ⟫ /\
   ⟪ FF  : F S' e ⟫ /\
   ⟪ JF' : jf S' ≡ jf S ⟫ /\
   ⟪ EW' : ew S' ≡ ew S ⟫ /\
   ⟪ CO' : co S' ≡ co S ⟫.
 
-Definition t_load
+Definition load_step
            (e  : eventid)
            (e' : option eventid)
            (S S' : ES.t) : Prop :=
   exists w, 
-    ⟪ ENONE : e' = None ⟫ /\
+    ⟪ nUPD : e' = None ⟫ /\
     ⟪ AJF : add_jf w e S S' ⟫ /\
     ⟪ EW' : ew S' ≡ ew S ⟫ /\
     ⟪ CO' : co S' ≡ co S ⟫.
 
-Definition t_store
+Definition store_step
            (e  : eventid)
            (e' : option eventid)
            (S S' : ES.t) : Prop :=
   exists ews ws, 
-    ⟪ ENONE : e' = None ⟫ /\
+    ⟪ nUPD : e' = None ⟫ /\
     ⟪ JF' : jf S' ≡ jf S ⟫ /\
     ⟪ AEW : add_ew ews e S S' ⟫ /\
     ⟪ ACO : add_co ews ws e S S' ⟫.
 
-Definition t_update
+Definition update_step
            (e  : eventid)
            (e' : option eventid)
            (S S' : ES.t) : Prop := 
   exists w ews ws w',
-    ⟪ ESOME : e' = Some w' ⟫ /\
+    ⟪ UPD : e' = Some w' ⟫ /\
     ⟪ AJF : add_jf w e S S' ⟫ /\
     ⟪ AEW : add_ew ews w' S S' ⟫ /\
     ⟪ ACO : add_co ews ws w' S S' ⟫.
 
-Definition t_ e e' S S' :=
-  t_fence e e' S S' \/ t_load e e' S S' \/ t_store e e' S S' \/ t_update e e' S S'.
+Definition step_ e e' S S' :=
+  fence_step e e' S S' \/ load_step e e' S S' \/ store_step e e' S S' \/ update_step e e' S S'.
 
-Definition t (m : model) (S S' : ES.t) : Prop := exists e e',
-  ⟪ TT  : t_ e e' S S' ⟫ /\
-  ⟪ BSTEP : ESBasicStep.t e e' S S' ⟫ /\
-  ⟪ CON : @es_consistent S' m ⟫.
+Definition step (m : model) (S S' : ES.t) : Prop := exists e e',
+  ⟪ TT : step_ e e' S S' ⟫ /\
+  ⟪ BSTEP : basic_step e e' S S' ⟫ /\
+  ⟪ CONS : @es_consistent S' m ⟫.
 
-(******************************************************************************)
-(** ** Deltas definitions *)
-(******************************************************************************)
+Ltac unfold_step_ H := 
+  unfold step_, 
+  fence_step, 
+  load_step, 
+  store_step, 
+  update_step 
+    in H; 
+  destruct H as [HA | [HB | [HC | HD]]]; desc.
 
-Definition jfi_delta S k w r : relation eventid := 
-  ⦗ES.cont_sb_dom S k⦘ ⨾ jf_delta w r.
-
-Definition jfe_delta S k w r : relation eventid := 
-  ⦗set_compl (ES.cont_sb_dom S k)⦘ ⨾ jf_delta w r.
-
-Definition sw_delta S S' k e e' : relation eventid := 
-  release S ⨾ (jf S ⨾ ESBasicStep.sb_delta S k e e' ⨾ ⦗F S'⦘ ∪ jf S' ⨾ ⦗eq e⦘) ⨾ ⦗Acq S'⦘.
-
-Definition hb_delta S S' k e e' : relation eventid := 
-  (hb S)^? ⨾ (ESBasicStep.sb_delta S k e e' ∪ sw_delta S S' k e e') ⨾ (eq e × eq_opt e')^? . 
-
-Hint Unfold jfi_delta jfe_delta sw_delta hb_delta : ESStepDb.
+Ltac unfold_step H := 
+  unfold step in H; 
+  destruct H as [H [BSTEP_ CONS]];
+  red in BSTEP_;
+  unfold_step_ H.
 
 (******************************************************************************)
-(** ** ews, ws, ws_compl lemmas *)
+(** ** Fence step properties *)
 (******************************************************************************)
 
-Lemma ewsEWLoc ews w' e e' S S'
-      (wf : ES.Wf S) 
-      (BSTEP : ESBasicStep.t e e' S S') 
-      (AEW : add_ew ews w' S S') : 
-  ews ⊆₁ (E S) ∩₁ (W S) ∩₁ (Loc_ S (loc S' w')).
-Proof. 
-  cdes AEW.
-  intros x xEWS.
-  unfolder; splits; auto.
-  etransitivity.
-  { symmetry. eapply ESBasicStep.basic_step_loc_eq_dom; eauto. }
-  symmetry. by apply ewsLOC in xEWS.
-Qed.
+Lemma fence_step_E e e' S S'
+      (BSTEP : basic_step e e' S S')
+      (FSTEP: fence_step e e' S S') :
+  E S' ≡₁ E S ∪₁ eq e.
+Proof. cdes FSTEP. subst. by apply basic_step_nupd_acts_set. Qed.
 
-Lemma ews_ew_fwcl ews w' S S'
-      (wf : ES.Wf S) 
-      (AEW : add_ew ews w' S S') : 
-  codom_rel (⦗ews⦘ ⨾ ew S) ⊆₁ ews.
-Proof.
-  cdes AEW. 
-  intros x [y [z [[EQz EWS] EW]]]. subst z.
-  apply ES.ew_sym in EW; auto.
-  apply ewsEWprcl.
-  basic_solver 10.
-Qed.
+Lemma fence_step_R e e' S S'
+      (BSTEP : basic_step e e' S S')
+      (FSTEP: fence_step e e' S S') 
+      (wfE: ES.Wf S) :
+  E S' ∩₁ R S' ≡₁ E S ∩₁ R S.
+Proof. cdes FSTEP. step_type_solver. Qed.  
 
-Lemma ws_co_prcl ews ws w' S S'
-      (wf : ES.Wf S) 
-      (ACO : add_co ews ws w' S S') : 
-  dom_rel (co S ⨾ ⦗ws⦘) ⊆₁ ws.
-Proof. cdes ACO. generalize wsCOEWprcl. basic_solver 10. Qed.
+Lemma fence_step_W e e' S S'
+      (BSTEP : basic_step e e' S S')
+      (FSTEP: fence_step e e' S S') 
+      (wfE: ES.Wf S) :
+  E S' ∩₁ W S' ≡₁ E S ∩₁ W S.
+Proof. cdes FSTEP. step_type_solver. Qed.  
 
-Lemma ws_ew_prcl ews ws w' S S'
-      (wf : ES.Wf S) 
-      (ACO : add_co ews ws w' S S') : 
-  dom_rel (ew S ⨾ ⦗ws⦘) ⊆₁ ws.
-Proof. cdes ACO. generalize wsCOEWprcl. basic_solver 10. Qed.
+Lemma fence_step_F e e' S S'
+      (BSTEP : basic_step e e' S S')
+      (FSTEP: fence_step e e' S S') 
+      (wfE: ES.Wf S) :
+  E S' ∩₁ F S' ≡₁ E S ∩₁ F S ∪₁ eq e.
+Proof. cdes FSTEP. step_type_solver. Qed.  
 
-Lemma ws_ew_fwcl ews ws w' S S'
-      (wf : ES.Wf S) 
-      (ACO : add_co ews ws w' S S') : 
-  codom_rel (⦗ws⦘ ⨾ ew S) ⊆₁ ws.
-Proof. 
-  cdes ACO. 
-  intros x [y [z [[EQz WS] EW]]]. subst z.
-  apply ES.ew_sym in EW; auto.
-  eapply ws_ew_prcl; eauto.
-  basic_solver 10.
-Qed.
+Lemma fence_step_acq e e' S S'
+      (BSTEP : basic_step e e' S S')
+      (FSTEP: fence_step e e' S S') 
+      (wfE: ES.Wf S) :
+  E S' ∩₁ FR S' ∩₁ Acq S' ≡₁ E S ∩₁ FR S ∩₁ Acq S ∪₁ eq e ∩₁ Acq S'.
+Proof. cdes FSTEP. step_type_solver. Qed.  
 
-Lemma ws_co_ew_prcl ews ws w' S S'
-      (wf : ES.Wf S) 
-      (ACO : add_co ews ws w' S S') : 
-  dom_rel (co S ⨾ ew S ⨾ ⦗ws⦘) ⊆₁ ws.
-Proof. cdes ACO. generalize wsCOEWprcl. basic_solver 10. Qed.
-
-Lemma ws_complE ews ws S 
-      (wf : ES.Wf S) : 
-  ws_compl ews ws S ⊆₁ E S.
-Proof. 
-  unfold ws_compl.
-  rewrite ES.coE; auto.
-  basic_solver.
-Qed.
-
-Lemma ws_complW ews ws S 
-      (wf : ES.Wf S) : 
-  ws_compl ews ws S ⊆₁ W S.
-Proof. 
-  unfold ws_compl.
-  rewrite ES.coD; auto.
-  basic_solver.
-Qed.
-
-Lemma ws_compl_loc ews ws w' e e' S S'
-      (wf : ES.Wf S) 
-      (BSTEP : ESBasicStep.t e e' S S') 
-      (AEW : add_ew ews w' S S')
-      (ACO : add_co ews ws w' S S') : 
-  ws_compl ews ws S ⊆₁ same_loc S' w'.
-Proof. 
-  cdes AEW; cdes ACO.
-  unfold ws_compl.
-  rewrite ES.coE; auto.
-  rewrite ewsLOC at 1.
-  rewrite wsLOC at 1.
-  rewrite ES.col; auto.
-  rewrite set_unionK.
-  intros x [[y HH] _].
-  unfolder in HH. desc.
-  etransitivity; eauto.
-  arewrite (loc S' y = loc S y).
-  { erewrite ESBasicStep.basic_step_loc_eq_dom; eauto. }
-  arewrite (loc S' x = loc S x).
-  { erewrite ESBasicStep.basic_step_loc_eq_dom; eauto. }
-  done. 
-Qed.
-
-Lemma wsEWLoc ews ws w' e e' S S'
-      (wf : ES.Wf S) 
-      (BSTEP : ESBasicStep.t e e' S S') 
-      (ACO : add_co ews ws w' S S') : 
-  ws ⊆₁ (E S) ∩₁ (W S) ∩₁ (Loc_ S (loc S' w')).
-Proof. 
-  cdes ACO.
-  intros x xWS.
-  unfolder; splits; auto.
-  etransitivity.
-  { symmetry. eapply ESBasicStep.basic_step_loc_eq_dom; eauto. }
-  symmetry. by apply wsLOC in xWS.
-Qed.
-
-Lemma ws_complEWLoc ews ws w' e e' S S'
-      (wf : ES.Wf S) 
-      (BSTEP : ESBasicStep.t e e' S S') 
-      (AEW : add_ew ews w' S S')
-      (ACO : add_co ews ws w' S S') : 
-  ws_compl ews ws S ⊆₁ (E S) ∩₁ (W S) ∩₁ (Loc_ S (loc S' w')).
-Proof. 
-  cdes ACO.
-  intros x xWS.
-  unfolder; splits; auto.
-  { eapply ws_complE; eauto. }
-  { eapply ws_complW; eauto. }
-  etransitivity.
-  { symmetry. eapply ESBasicStep.basic_step_loc_eq_dom; eauto. 
-    eapply ws_complE; eauto. }
-  symmetry. eapply ws_compl_loc in xWS; eauto. 
-Qed.
-
-Lemma ws_compl_co_fwcl ews ws w' S S'
-      (wf : ES.Wf S) 
-      (ACO : add_co ews ws w' S S') : 
-  codom_rel (⦗ws_compl ews ws S⦘ ⨾ co S) ⊆₁ ws_compl ews ws S.
-Proof. 
-  cdes ACO. 
-  unfold ws_compl. 
-  intros y [x [z [[EQz HH] CO]]]. subst z.
-  destruct HH as [[z [z' [[EQz' EWWS] COzx]]] nEWWS]. subst z'.
-  red. splits.
-  { do 2 eexists. splits. 
-    { red. eauto using EWWS. }
-    eapply ES.co_trans; eauto. }
-  intros EWWSy. apply nEWWS.
-  generalize wsCOEWprcl ewsCOprcl EWWSy CO.
-  basic_solver 10.
-Qed.
-
-Lemma ws_compl_ew_fwcl ews ws w' S S'
-      (wf : ES.Wf S) 
-      (AEW : add_ew ews w' S S')
-      (ACO : add_co ews ws w' S S') : 
-  codom_rel (⦗ws_compl ews ws S⦘ ⨾ ew S) ⊆₁ ws_compl ews ws S.
-Proof. 
-  cdes AEW; cdes ACO. 
-  unfold ws_compl. 
-  intros y [x [z [[EQz HH] EW]]]. subst z.
-  destruct HH as [[z [z' [[EQz' EWWS] COzx]]] nEWWS]. subst z'.
-  red. splits.
-  { do 2 eexists. splits. 
-    { red. eauto using EWWS. }
-    eapply ES.co_ew_in_co; eauto. 
-    basic_solver. }
-  intros EWWSy. apply nEWWS.
-  generalize wsCOEWprcl ewsCOprcl EWWSy ewsEWprcl EW.
-  basic_solver 10.
-Qed.
-
-Lemma ws_inter_ws_compl_false ews ws w' S S'
-      (wf : ES.Wf S) 
-      (ACO : add_co ews ws w' S S') : 
-  ws ∩₁ ws_compl ews ws S ⊆₁ ∅.
-Proof. unfold ws_compl. basic_solver. Qed.
-
-Lemma ews_inter_ws_compl_false ews ws w' S S'
-      (wf : ES.Wf S) 
-      (ACO : add_co ews ws w' S S') : 
-  ews ∩₁ ws_compl ews ws S ⊆₁ ∅.
-Proof. unfold ws_compl. basic_solver. Qed.
-
-Lemma ws_cross_ws_compl_in_co ews ws w' e e' S S'
-      (wf : ES.Wf S) 
-      (BSTEP : ESBasicStep.t e e' S S') 
-      (AEW : add_ew ews w' S S')
-      (ACO : add_co ews ws w' S S') 
-      (wEE' : (eq e ∪₁ eq_opt e') w') : 
-  ws × ws_compl ews ws S ⊆ co S.
-Proof. 
-  cdes AEW; cdes ACO.
-  intros x y [xWS yWS].
-  destruct 
-    (excluded_middle_informative (ew S x y))
-    as [EW | nEW].
-  { exfalso.
-    destruct yWS as [HH nEWWS].
-    eapply nEWWS.
-    right. eapply ws_ew_fwcl; eauto. 
-    basic_solver 10. }
-  edestruct ES.co_total; eauto.
-  { eapply wsEWLoc; eauto. }
-  { eapply ws_complEWLoc; eauto. }
-  exfalso. 
-  destruct yWS as [HH nEWWS].
-  apply nEWWS.
-  right. eapply ws_co_prcl; eauto.
-  basic_solver 10. 
-Qed.
-
-Lemma ws_cross_ews_in_ew_compl ews ws w' e e' S S'
-      (wf : ES.Wf S)
-      (BSTEP : ESBasicStep.t e e' S S')
-      (AEW : add_ew ews w' S S')
-      (ACO : add_co ews ws w' S S')
-      (wEE' : (eq e ∪₁ eq_opt e') w') :
-  ws × ews ⊆ compl_rel (ew S).
-Proof.
-  cdes AEW; cdes ACO.
-  intros x y [xWS yEWS].
-  assert (~ ews x) as xnEWS.
-  { red. ins. eapply ws_ews; eauto. basic_solver. }
-  intros EW. eapply ws_ews; eauto.
-  split; [|eauto].
-  eapply ws_ew_fwcl; eauto.
-  basic_solver 10.
-Qed.
-
-Lemma ews_cross_ws_compl_in_ew_compl ews ws w' e e' S S'
-      (wf : ES.Wf S) 
-      (BSTEP : ESBasicStep.t e e' S S') 
-      (AEW : add_ew ews w' S S')
-      (ACO : add_co ews ws w' S S') 
-      (wEE' : (eq e ∪₁ eq_opt e') w') : 
-  ews × ws_compl ews ws S ⊆ compl_rel (ew S).
-Proof. 
-  cdes AEW; cdes ACO.
-  intros x y [xEWS yWSC].
-  assert (~ ews y) as ynEWS.
-  { red. ins. eapply ews_inter_ws_compl_false; eauto. basic_solver. }
-  intros EW. eapply ews_inter_ws_compl_false; eauto.
-  split; [|eauto].
-  eapply ews_ew_fwcl; eauto.
-  basic_solver 10.
-Qed.
-
-Lemma ws_cross_ews_in_co ews ws w' e e' S S'
-      (wf : ES.Wf S) 
-      (BSTEP : ESBasicStep.t e e' S S') 
-      (AEW : add_ew ews w' S S')
-      (ACO : add_co ews ws w' S S') 
-      (wEE' : (eq e ∪₁ eq_opt e') w') : 
-  ws × ews ⊆ co S.
-Proof. 
-  cdes AEW; cdes ACO.
-  intros x y [xWS yEWS].
-  assert (~ ew S x y) as nEW.
-  { eapply ws_cross_ews_in_ew_compl; eauto. basic_solver. }
-  edestruct ES.co_total as [COxy | COyx]; eauto.
-  { eapply wsEWLoc; eauto. }
-  { eapply ewsEWLoc; eauto. }
-  exfalso. eapply ws_ews.
-  split; [|eauto].
-  eapply ws_co_prcl; eauto.
-  basic_solver 10.
-Qed.
-
-Lemma ews_cross_ws_compl_in_co ews ws w' e e' S S'
-      (wf : ES.Wf S) 
-      (BSTEP : ESBasicStep.t e e' S S') 
-      (AEW : add_ew ews w' S S')
-      (ACO : add_co ews ws w' S S') 
-      (wEE' : (eq e ∪₁ eq_opt e') w') : 
-  ews × ws_compl ews ws S ⊆ co S.
-Proof. 
-  cdes AEW; cdes ACO.
-  intros x y [xEWS yWSC].
-  assert (~ ew S x y) as nEW.
-  { eapply ews_cross_ws_compl_in_ew_compl; eauto. basic_solver. }
-  set (yWSC' := yWSC).
-  destruct yWSC' as [[z [z' [[EQz' HA] CO]]] HB]. subst z'.
-  destruct HA as [zEWS | zWS].
-  { apply ES.ew_co_in_co; auto.
-    eexists; splits; eauto. 
-    apply ewsEW. basic_solver. }
-  edestruct ES.co_total as [COxy | COyx]; eauto.
-  { eapply ewsEWLoc; eauto. }
-  { eapply ws_complEWLoc; eauto. }
-  exfalso. eapply HB.
-  right. apply ewsCOprcl. basic_solver 10.
-Qed.
-
-Lemma ews_co_codom ews ws w' S S'
-      (wf : ES.Wf S) 
-      (AEW : add_ew ews w' S S')
-      (ACO : add_co ews ws w' S S') : 
-  codom_rel (⦗ews⦘ ⨾ co S) ⊆₁ ws_compl ews ws S. 
-Proof. 
-  cdes AEW; cdes ACO.
-  unfold ws_compl.
-  intros x [y [z [[EQz EWS] CO]]]. subst z.
-  unfolder; splits; eauto 10.
-  intros [EW | WS].
-  { eapply ES.ew_co; eauto.
-    split; eauto.
-    eapply ewsEW. 
-    basic_solver. }
-  eapply ws_ews. split; [|eauto].
-  eapply ws_co_prcl; eauto. basic_solver 10. 
-Qed.
-
-Lemma ews_co_ws_empty ews ws w' S S'
-      (wf : ES.Wf S) 
-      (AEW : add_ew ews w' S S')
-      (ACO : add_co ews ws w' S S') : 
-  ⦗ews⦘ ⨾ co S ⨾ ⦗ws⦘ ⊆ ∅₂.
-Proof. 
-  cdes AEW; cdes ACO.
-  rewrite <- seqA.
-  intros x y [z [HA [EQz WSy]]]. subst z.
-  eapply ws_inter_ws_compl_false; eauto.
-  split; eauto.
-  eapply ews_co_codom; eauto.
-  basic_solver.
-Qed.
+Lemma fence_step_Rel e e' S S'
+      (BSTEP : basic_step e e' S S')
+      (FSTEP: fence_step e e' S S') 
+      (wfE: ES.Wf S) :
+  E S' ∩₁ FW S' ∩₁ Rel S' ≡₁ E S ∩₁ FW S ∩₁ Rel S ∪₁ eq e ∩₁ Rel S'.
+Proof. cdes FSTEP. step_type_solver. Qed.  
 
 (******************************************************************************)
-(** ** Deltas lemmas *)
+(** ** Load step properties *)
 (******************************************************************************)
 
-Lemma step_add_jf_jf_delta_dom w e e' S S'
-      (BSTEP : ESBasicStep.t e e' S S') 
-      (AJF : add_jf w e S S') 
-      (wf : ES.Wf S) : 
-  dom_rel (jf_delta w e) ⊆₁ E S.
-Proof. 
-  cdes AJF; cdes BSTEP; cdes BSTEP_.
-  ESBasicStep.step_solver.
-Qed.  
+Lemma load_step_E e e' S S'
+      (BSTEP : basic_step e e' S S')
+      (LSTEP: load_step e e' S S') :
+  E S' ≡₁ E S ∪₁ eq e.
+Proof. cdes LSTEP. subst. by apply basic_step_nupd_acts_set. Qed.
 
-Lemma step_add_jf_jf_deltaE w e e' S S'
-      (BSTEP : ESBasicStep.t e e' S S') 
-      (AJF : add_jf w e S S') 
-      (wf : ES.Wf S) : 
-  jf_delta w e ⨾ ⦗E S⦘ ≡ ∅₂. 
-Proof. 
-  cdes AJF; cdes BSTEP; cdes BSTEP_.
-  split; [|done].
-  ESBasicStep.step_solver.
-Qed.  
-
-Lemma step_add_jf_jfi_delta_dom lang k k' st st' w e e' S S'
-      (BSTEP_ : ESBasicStep.t_ lang k k' st st' e e' S S') 
-      (AJF : add_jf w e S S') 
-      (wf : ES.Wf S) : 
-  dom_rel (jfi_delta S k w e) ⊆₁ E S.
-Proof. 
-  cdes AJF; cdes BSTEP_.
-  ESBasicStep.step_solver.
-Qed.  
-
-Lemma step_add_jf_jfe_delta_dom lang k k' st st' w e e' S S'
-      (BSTEP_ : ESBasicStep.t_ lang k k' st st' e e' S S') 
-      (AJF : add_jf w e S S') 
-      (wf : ES.Wf S) : 
-  dom_rel (jfe_delta S k w e) ⊆₁ E S.
-Proof. 
-  cdes AJF; cdes BSTEP_.
-  ESBasicStep.step_solver.
-Qed.
-
-Lemma step_add_jf_jfi_deltaE lang k k' st st' w e e' S S'
-      (BSTEP_ : ESBasicStep.t_ lang k k' st st' e e' S S') 
-      (AJF : add_jf w e S S') 
-      (wf : ES.Wf S) : 
-  jfi_delta S k w e ⨾ ⦗E S⦘ ≡ ∅₂.
-Proof. 
-  cdes AJF; cdes BSTEP_.
-  split; [|done].
-  ESBasicStep.step_solver.
-Qed.  
-
-Lemma step_add_jf_jfe_deltaE lang k k' st st' w e e' S S'
-      (BSTEP_ : ESBasicStep.t_ lang k k' st st' e e' S S') 
-      (AJF : add_jf w e S S') 
-      (wf : ES.Wf S) : 
-  jfe_delta S k w e ⨾ ⦗E S⦘ ≡ ∅₂.
-Proof. 
-  cdes AJF; cdes BSTEP_.
-  split; [|done].
-  ESBasicStep.step_solver.
-Qed.  
-
-Lemma step_add_ew_ew_delta_dom ews w' e e' S S'
-      (BSTEP : ESBasicStep.t e e' S S') 
-      (AEW : add_ew ews w' S S') 
-      (wf : ES.Wf S) 
-      (wEE' : (eq e ∪₁ eq_opt e') w') : 
-  dom_rel (ew_delta ews w') ⊆₁ ews ∪₁ eq w'.
-Proof. unfold ew_delta. basic_solver. Qed.
-
-Lemma step_add_ew_ew_delta_codom ews w' e e' S S'
-      (BSTEP : ESBasicStep.t e e' S S') 
-      (AEW : add_ew ews w' S S') 
-      (wf : ES.Wf S) 
-      (wEE' : (eq e ∪₁ eq_opt e') w') : 
-  codom_rel (ew_delta ews w') ⊆₁ ews ∪₁ eq w'.
-Proof. unfold ew_delta. basic_solver. Qed.
-
-Lemma step_add_ew_ew_deltaEl ews w' e e' S S'
-      (BSTEP : ESBasicStep.t e e' S S') 
-      (AEW : add_ew ews w' S S') 
-      (wf : ES.Wf S) 
-      (wEE' : (eq e ∪₁ eq_opt e') w') : 
-  ew_delta ews w' ⨾ ⦗E S⦘ ≡ eq w' × ews. 
-Proof. 
-  cdes AEW; cdes BSTEP; cdes BSTEP_.
-  unfold ew_delta. 
-  rewrite csE, transp_cross.
-  relsf.
-  arewrite_false (eq w' × eq w' ⨾ ⦗E S⦘).
-  { unfolder in wEE'; desf; ESBasicStep.step_solver. }
-  arewrite_false (ews × eq w' ⨾ ⦗E S⦘).
-  { unfolder in wEE'; desf; ESBasicStep.step_solver. }
-  relsf. 
-  generalize ewsE. basic_solver.
-Qed.
-
-Lemma step_add_ew_ew_deltaEr ews w' e e' S S'
-      (BSTEP : ESBasicStep.t e e' S S') 
-      (AEW : add_ew ews w' S S') 
-      (wf : ES.Wf S) 
-      (wEE' : (eq e ∪₁ eq_opt e') w') : 
-  ⦗E S⦘ ⨾ ew_delta ews w' ≡ ews × eq w'. 
-Proof. 
-  cdes AEW; cdes BSTEP; cdes BSTEP_.
-  unfold ew_delta. 
-  rewrite csE, transp_cross.
-  relsf.
-  arewrite_false (⦗E S⦘ ⨾ eq w' × eq w').
-  { unfolder in wEE'; desf; ESBasicStep.step_solver. }
-  arewrite_false (⦗E S⦘ ⨾ eq w' × ews).
-  { unfolder in wEE'; desf; ESBasicStep.step_solver. }
-  relsf. 
-  generalize ewsE. basic_solver.
-Qed.
-
-Lemma step_add_co_co_delta_dom ews ws w' e e' S S'
-      (BSTEP : ESBasicStep.t e e' S S') 
-      (ACO : add_co ews ws w' S S') 
-      (wf : ES.Wf S) 
-      (wEE' : (eq e ∪₁ eq_opt e') w') : 
-  dom_rel (co_delta ews ws w' S) ⊆₁ ws ∪₁ eq w'.
-Proof. unfold co_delta. basic_solver. Qed.
-
-Lemma step_add_co_co_delta_codom ews ws w' e e' S S'
-      (BSTEP : ESBasicStep.t e e' S S') 
-      (ACO : add_co ews ws w' S S') 
-      (wf : ES.Wf S) 
-      (wEE' : (eq e ∪₁ eq_opt e') w') : 
-  codom_rel (co_delta ews ws w' S) ⊆₁ ws_compl ews ws S ∪₁ eq w'.
-Proof. unfold co_delta. basic_solver. Qed.
-
-Lemma step_add_co_co_deltaEl ews ws w' e e' S S'
-      (BSTEP : ESBasicStep.t e e' S S') 
-      (ACO : add_co ews ws w' S S') 
-      (wf : ES.Wf S) 
-      (wEE' : (eq e ∪₁ eq_opt e') w') : 
-  co_delta ews ws w' S ⨾ ⦗E S⦘ ≡ eq w' × ws_compl ews ws S.
-Proof. 
-  cdes ACO; cdes BSTEP; cdes BSTEP_.
-  unfold co_delta. relsf.
-  arewrite_false (ws × eq w' ⨾ ⦗E S⦘).
-  { unfolder in wEE'; desf; ESBasicStep.step_solver. }
-  relsf. split; [basic_solver|].
-  unfolder. ins. desf. splits; auto.
-  eapply ws_complE; eauto.
-Qed.  
-
-Lemma step_add_co_co_deltaEr ews ws w' e e' S S'
-      (BSTEP : ESBasicStep.t e e' S S') 
-      (ACO : add_co ews ws w' S S') 
-      (wf : ES.Wf S) 
-      (wEE' : (eq e ∪₁ eq_opt e') w') : 
-  ⦗E S⦘ ⨾ co_delta ews ws w' S ≡ ws × eq w'.
-Proof. 
-  cdes ACO; cdes BSTEP; cdes BSTEP_.
-  unfold co_delta. relsf.
-  arewrite_false (⦗E S⦘ ⨾ eq w' × ws_compl ews ws S). 
-  { unfolder in wEE'; desf; ESBasicStep.step_solver. }
-  basic_solver 10.
-Qed.  
-
-Lemma basic_step_sw_delta_dom lang k k' st st' e e' S S'
-      (BSTEP_ : ESBasicStep.t_ lang k k' st st' e e' S S') 
+Lemma load_step_R e e' S S'
+      (BSTEP : basic_step e e' S S')
+      (LSTEP: load_step e e' S S') 
       (wfE: ES.Wf S) :
-  dom_rel (sw_delta S S' k e e') ⊆₁ E S.
-Proof. 
-  cdes BSTEP_.
-  ESBasicStep.step_solver.
-Qed.
+  E S' ∩₁ R S' ≡₁ E S ∩₁ R S ∪₁ eq e.
+Proof. cdes LSTEP; cdes AJF. step_type_solver. Qed.  
 
-Lemma basic_step_sw_deltaE lang k k' st st' e e' S S'
-      (BSTEP_ : ESBasicStep.t_ lang k k' st st' e e' S S') 
+Lemma load_step_W e e' S S'
+      (BSTEP : basic_step e e' S S')
+      (LSTEP: load_step e e' S S') 
       (wfE: ES.Wf S) :
-  sw_delta S S' k e e' ⨾ ⦗E S⦘ ≡ ∅₂.
-Proof. 
-  cdes BSTEP_.
-  split; [|done]. 
-  unfold sw_delta.
-  ESBasicStep.step_solver.
-Qed.
+  E S' ∩₁ W S' ≡₁ E S ∩₁ W S.
+Proof. cdes LSTEP; cdes AJF. step_type_solver. Qed.  
 
-Lemma basic_step_hb_delta_dom lang k k' st st' e e' S S' 
-      (BSTEP_ : ESBasicStep.t_ lang k k' st st' e e' S S') 
+Lemma load_step_F e e' S S'
+      (BSTEP : basic_step e e' S S')
+      (LSTEP: load_step e e' S S') 
       (wfE: ES.Wf S) :
-  dom_rel (hb_delta S S' k e e') ⊆₁ E S ∪₁ eq e.
-Proof. 
-  cdes BSTEP_.
-  unfold hb_delta.
-  rewrite crE, !seq_union_l, seq_id_l. 
-  rewrite !dom_union, !dom_seq.
-  rewrite !set_subset_union_l.
-  splits. 
-  { eapply ESBasicStep.basic_step_sb_delta_dom; eauto. }
-  all : ESBasicStep.step_solver.
-Qed. 
+  E S' ∩₁ F S' ≡₁ E S ∩₁ F S.
+Proof. cdes LSTEP; cdes AJF. step_type_solver. Qed.  
 
-Lemma basic_step_hb_deltaE lang k k' st st' e e' S S' 
-      (BSTEP_ : ESBasicStep.t_ lang k k' st st' e e' S S') 
+Lemma load_step_acq e e' S S'
+      (BSTEP : basic_step e e' S S')
+      (LSTEP: load_step e e' S S') 
       (wfE: ES.Wf S) :
-  hb_delta S S' k e e' ⨾ ⦗E S⦘ ≡ ∅₂.
-Proof. 
-  cdes BSTEP_.
-  split; [|done].
-  ESBasicStep.step_solver.
-Qed.
+  E S' ∩₁ FR S' ∩₁ Acq S' ≡₁ E S ∩₁ FR S ∩₁ Acq S ∪₁ eq e ∩₁ Acq S'.
+Proof. cdes LSTEP; cdes AJF. step_type_solver. Qed.  
 
-Lemma basic_step_hb_delta_alt lang k k' st st' e e' S S'
-      (BSTEP_ : ESBasicStep.t_ lang k k' st st' e e' S S') 
+Lemma load_step_Rel e e' S S'
+      (BSTEP : basic_step e e' S S')
+      (LSTEP: load_step e e' S S') 
       (wfE: ES.Wf S) :
-  hb_delta S S' k e e' ≡ 
-    (hb S)^? ⨾ ((ESBasicStep.sb_delta S k e e' ∪ sw_delta S S' k e e') ⨾ (hb S)^?)⁺.
-Proof. 
-  cdes BSTEP_.
-  unfold hb_delta. 
-  apply seq_more; auto.
-  rewrite !crE. relsf.
-  rewrite hbE; auto.
-  arewrite_false (ESBasicStep.sb_delta S k e e' ⨾ ⦗E S⦘).
-  { eapply ESBasicStep.basic_step_sb_deltaE; eauto. }
-  arewrite_false (sw_delta S S' k e e' ⨾ ⦗E S⦘).
-  { eapply basic_step_sw_deltaE; eauto. }
-  relsf.
-  rewrite ct_begin, rtE. relsf.
-  rewrite !unionA.
-  do 3 (apply union_more; auto).
-  { rewrite ct_begin, rtE. relsf.
-    rewrite <- !seqA.
-    arewrite_false (ESBasicStep.sb_delta S k e e' ⨾ sw_delta S S' k e e'). 
-    { ESBasicStep.step_solver. }
-    rewrite <- !seqA.
-    arewrite 
-      (ESBasicStep.sb_delta S k e e' ⨾ ESBasicStep.sb_delta S k e e' ≡ 
-                            ESBasicStep.sb_delta S k e e' ⨾ eq e × eq_opt e').
-    { rewrite dom_rel_helper with (r := ESBasicStep.sb_delta S k e e') at 2.
-      2 : eapply ESBasicStep.basic_step_sb_delta_dom; eauto.
-      rewrite id_union. relsf. 
-      arewrite_false (ESBasicStep.sb_delta S k e e' ⨾ ⦗E S⦘).
-      { ESBasicStep.step_solver. }
-      relsf.
-      apply seq_more; auto.
-      unfold ESBasicStep.sb_delta. 
-      rewrite cross_union_r. relsf.
-      arewrite_false (⦗eq e⦘ ⨾ ES.cont_sb_dom S k × eq e). 
-      { ESBasicStep.step_solver. }
-      arewrite_false (⦗eq e⦘ ⨾ ES.cont_sb_dom S k × eq_opt e'). 
-      { ESBasicStep.step_solver. }
-      basic_solver 20. }
-    relsf.
-    rewrite ct_begin, rtE. relsf.
-
-    arewrite_false (eq e × eq_opt e' ⨾ ESBasicStep.sb_delta S k e e').
-    { ESBasicStep.step_solver. }
-    arewrite_false (eq e × eq_opt e' ⨾ ESBasicStep.sb_delta S k e e').
-    { ESBasicStep.step_solver. }
-    arewrite_false (eq e × eq_opt e' ⨾ sw_delta S S' k e e').
-    { ESBasicStep.step_solver. }
-    arewrite_false (eq e × eq_opt e' ⨾ sw_delta S S' k e e').
-    { ESBasicStep.step_solver. }
-    basic_solver 10. }
-
-  rewrite ct_begin, rtE. relsf.
-  rewrite <- !seqA.
-  arewrite_false (sw_delta S S' k e e' ⨾ sw_delta S S' k e e'). 
-  { unfold sw_delta. ESBasicStep.step_solver. }
-  rewrite <- !seqA.
-  arewrite 
-    (sw_delta S S' k e e' ⨾ ESBasicStep.sb_delta S k e e' ≡ 
-              sw_delta S S' k e e' ⨾ eq e × eq_opt e').
-  { rewrite dom_rel_helper with (r := ESBasicStep.sb_delta S k e e').
-    2 : eapply ESBasicStep.basic_step_sb_delta_dom; eauto.
-    rewrite id_union. relsf. 
-    arewrite_false (sw_delta S S' k e e' ⨾ ⦗E S⦘).
-    { unfold sw_delta. ESBasicStep.step_solver. }
-    unfold ESBasicStep.sb_delta. 
-    rewrite cross_union_r. relsf.
-    arewrite_false (⦗eq e⦘ ⨾ ES.cont_sb_dom S k × eq e).
-    { ESBasicStep.step_solver. }
-    arewrite_false (⦗eq e⦘ ⨾ ES.cont_sb_dom S k × eq_opt e').
-    { ESBasicStep.step_solver. }
-    basic_solver 10. }
-  
-  relsf.
-  rewrite ct_begin, rtE. relsf.
-  arewrite_false (eq e × eq_opt e' ⨾ ESBasicStep.sb_delta S k e e').
-  { ESBasicStep.step_solver. }
-  arewrite_false (eq e × eq_opt e' ⨾ ESBasicStep.sb_delta S k e e').
-  { ESBasicStep.step_solver. }
-  arewrite_false (eq e × eq_opt e' ⨾ sw_delta S S' k e e').
-  { ESBasicStep.step_solver. }
-  arewrite_false (eq e × eq_opt e' ⨾ sw_delta S S' k e e').
-  { ESBasicStep.step_solver. }
-  basic_solver 10.   
-Qed.
+  E S' ∩₁ FW S' ∩₁ Rel S' ≡₁ E S ∩₁ FW S ∩₁ Rel S.
+Proof. cdes LSTEP; cdes AJF. step_type_solver. Qed.  
 
 (******************************************************************************)
-(** ** Auxiliary lemmas *)
+(** ** Store step properties *)
 (******************************************************************************)
 
-Lemma basic_step_w_sb_loc_wE e e' S S'
-      (BSTEP : ESBasicStep.t e e' S S') 
+Lemma store_step_E e e' S S'
+      (BSTEP : basic_step e e' S S')
+      (SSTEP: store_step e e' S S') :
+  E S' ≡₁ E S ∪₁ eq e.
+Proof. cdes SSTEP. subst. by apply basic_step_nupd_acts_set. Qed.
+
+Lemma store_step_R e e' S S'
+      (BSTEP : basic_step e e' S S')
+      (SSTEP: store_step e e' S S') 
       (wfE: ES.Wf S) :
-  ⦗E S' ∩₁ W S'⦘ ⨾ (sb S' ∩ same_loc S')^? ⨾ ⦗W S'⦘ ⨾ ⦗E S⦘ ≡ 
-  ⦗E S  ∩₁ W S ⦘ ⨾ (sb S  ∩ same_loc S )^? ⨾ ⦗W S ⦘.
-Proof. 
-  cdes BSTEP. cdes BSTEP_.
-  arewrite (⦗W S'⦘ ⨾ ⦗E S⦘ ≡ ⦗E S⦘ ⨾ ⦗W S⦘). 
-  { rewrite seq_eqvC.
-    rewrite !seq_eqv.
-    apply eqv_rel_more.
-    eapply ESBasicStep.type_step_eq_dom; eauto. }
-  arewrite ((sb S' ∩ same_loc S')^? ⨾ ⦗E S⦘ ≡ ⦗E S⦘ ⨾ (sb S ∩ same_loc S)^?).
-  { rewrite !crE. relsf.
-    apply union_more; auto.
-    rewrite <- lib.AuxRel.seq_eqv_inter_lr.
-    rewrite ESBasicStep.basic_step_sbE; eauto.
-    rewrite ES.sbE at 1; auto.
-    rewrite <- restr_relE, <- restr_inter_absorb_r.
-    rewrite ESBasicStep.basic_step_same_loc_restr; eauto.
-    rewrite restr_inter_absorb_r, restr_relE.
-    rewrite ES.sbE; auto.
-    basic_solver 20. }
-  arewrite (⦗E S' ∩₁ W S'⦘ ⨾ ⦗E S⦘ ≡ ⦗E S ∩₁ W S⦘).
-  { rewrite ESBasicStep.basic_step_acts_set; eauto.
-    rewrite !set_inter_union_l, !id_union. relsf.
-    arewrite_false (⦗eq e ∩₁ W S'⦘ ⨾ ⦗E S⦘).
-    { ESBasicStep.step_solver. }
-    arewrite_false (⦗eq_opt e' ∩₁ W S'⦘ ⨾ ⦗E S⦘).
-    { ESBasicStep.step_solver. }
-    relsf. 
-    arewrite (E S ∩₁ W S' ≡₁ E S ∩₁ W S).
-    { eapply ESBasicStep.type_step_eq_dom; eauto. }
-    basic_solver. }
-  done.
-Qed.
+  E S' ∩₁ R S' ≡₁ E S ∩₁ R S.
+Proof. cdes SSTEP; cdes ACO. step_type_solver. Qed.  
 
-(*******************************************************)
-(* Lemmas about equality of types and modes of events
-   after a basic step.                                 *)
-(*******************************************************)
-
-Hint Unfold eq_dom Events.loc Events.val Events.mod Events.xmod 
-     is_r is_w is_f is_acq is_rel is_rlx is_acqrel R_ex
-     is_only_pln is_sc is_ra is_xacq
-     same_lab_u2v_dom same_label_u2v :
-  same_lab_unfoldDb.
-
-Ltac basic_step_same_lab S S' :=
-  repeat autounfold with same_lab_unfoldDb;
-  intros x [EX REL];
-  assert (lab S' x = lab S x) as HH;
-  [eapply ESBasicStep.basic_step_lab_eq_dom; eauto |
-    try (by rewrite HH in REL);
-    try (by rewrite <- HH in REL)].
-
-Lemma basic_step_mod_in_mod e e' S S'
-      (BSTEP : ESBasicStep.t e e' S S') :
-  forall l, E S ∩₁ Mod_ S' l ⊆₁ Mod_ S l.
-Proof. ins. basic_step_same_lab S S'. Qed.
-
-Lemma basic_step_loc_in_loc e e' S S'
-      (BSTEP : ESBasicStep.t e e' S S') :
-  forall l, E S ∩₁ Loc_ S' l ⊆₁ Loc_ S l.
-Proof. ins. basic_step_same_lab S S'. Qed.
-
-Lemma basic_step_val_in_val e e' S S'
-      (BSTEP : ESBasicStep.t e e' S S') :
-  forall v, E S ∩₁ Val_ S' v ⊆₁ Val_ S v.
-Proof. ins. basic_step_same_lab S S'. Qed.
-
-Lemma basic_step_rel_in_rel e e' S S'
-      (BSTEP : ESBasicStep.t e e' S S') :
-  E S ∩₁ Rel S' ⊆₁ Rel S.
-Proof. basic_step_same_lab S S'. Qed.
-
-Lemma basic_step_acq_in_acq e e' S S'
-      (BSTEP : ESBasicStep.t e e' S S') :
-  E S ∩₁ Acq S' ⊆₁ Acq S.
-Proof. basic_step_same_lab S S'. Qed.
-
-Lemma basic_step_sc_in_sc e e' S S'
-      (BSTEP : ESBasicStep.t e e' S S') :
-  E S ∩₁ Sc S' ⊆₁ Sc S.
-Proof. basic_step_same_lab S S'. Qed.
-
-Lemma basic_step_r_in_r e e' S S'
-      (BSTEP : ESBasicStep.t e e' S S') :
-  E S ∩₁ R S' ⊆₁ R S.
-Proof. basic_step_same_lab S S'. Qed.
-
-Lemma basic_step_w_in_w e e' S S'
-      (BSTEP : ESBasicStep.t e e' S S') :
-  E S ∩₁ W S' ⊆₁ W S.
-Proof. basic_step_same_lab S S'. Qed.
-
-Lemma basic_step_f_in_f e e' S S'
-      (BSTEP : ESBasicStep.t e e' S S') :
-  E S ∩₁ F S' ⊆₁ F S.
-Proof. basic_step_same_lab S S'. Qed.
-
-Lemma basic_step_rel_eq_rel e e' S S'
-      (BSTEP : ESBasicStep.t e e' S S') :
-  E S ∩₁ Rel S' ≡₁ E S ∩₁ Rel S.
-Proof. split; basic_step_same_lab S S'. Qed.
-
-Lemma basic_step_acq_eq_acq e e' S S'
-      (BSTEP : ESBasicStep.t e e' S S') :
-  E S ∩₁ Acq S' ≡₁ E S ∩₁ Acq S.
-Proof. split; basic_step_same_lab S S'. Qed.
-
-Lemma basic_step_sc_eq_sc e e' S S'
-      (BSTEP : ESBasicStep.t e e' S S') :
-  E S ∩₁ Sc S' ≡₁ E S ∩₁ Sc S.
-Proof. split; basic_step_same_lab S S'. Qed.
-
-Lemma basic_step_r_eq_r e e' S S'
-      (BSTEP : ESBasicStep.t e e' S S') :
-  E S ∩₁ R S' ≡₁ E S ∩₁ R S.
-Proof. split; basic_step_same_lab S S'. Qed.
-
-Lemma basic_step_w_eq_w e e' S S'
-      (BSTEP : ESBasicStep.t e e' S S') :
-  E S ∩₁ W S' ≡₁ E S ∩₁ W S.
-Proof. split; basic_step_same_lab S S'. Qed.
-
-Lemma basic_step_f_eq_f e e' S S'
-      (BSTEP : ESBasicStep.t e e' S S') :
-  E S ∩₁ F S' ≡₁ E S ∩₁ F S.
-Proof. split; basic_step_same_lab S S'. Qed.
-
-Lemma basic_step_fr_eq_fr e e' S S'
-      (BSTEP : ESBasicStep.t e e' S S') :
-  E S ∩₁ FR S' ≡₁ E S ∩₁ FR S.
-Proof. 
-  rewrite !set_inter_union_r.
-  erewrite basic_step_f_eq_f; eauto. 
-  erewrite basic_step_r_eq_r; eauto. 
-Qed.
-
-Lemma basic_step_fw_eq_fw e e' S S'
-      (BSTEP : ESBasicStep.t e e' S S') :
-  E S ∩₁ FW S' ≡₁ E S ∩₁ FW S.
-Proof. 
-  rewrite !set_inter_union_r.
-  erewrite basic_step_f_eq_f; eauto. 
-  erewrite basic_step_w_eq_w; eauto. 
-Qed.
-
-Lemma basic_step_fracq_eq_fracq e e' S S'
-      (BSTEP : ESBasicStep.t e e' S S') :
-  E S ∩₁ FR S' ∩₁ Acq S' ≡₁ E S ∩₁ FR S ∩₁ Acq S.
-Proof. 
-  erewrite basic_step_fr_eq_fr; eauto. 
-  arewrite (E S ∩₁ FR S ∩₁ Acq S' ≡₁ E S ∩₁ Acq S' ∩₁ FR S).
-  { basic_solver. }
-  erewrite basic_step_acq_eq_acq; eauto. 
-  basic_solver.
-Qed.
-
-Lemma basic_step_fwrel_eq_fwrel e e' S S'
-      (BSTEP : ESBasicStep.t e e' S S') :
-  E S ∩₁ FW S' ∩₁ Rel S' ≡₁ E S ∩₁ FW S ∩₁ Rel S.
-Proof. 
-  erewrite basic_step_fw_eq_fw; eauto. 
-  arewrite (E S ∩₁ FW S ∩₁ Rel S' ≡₁ E S ∩₁ Rel S' ∩₁ FW S).
-  { basic_solver. }
-  erewrite basic_step_rel_eq_rel; eauto. 
-  basic_solver.
-Qed.
-
-Hint Rewrite
-     basic_step_rel_in_rel
-     basic_step_acq_in_acq
-     basic_step_sc_in_sc
-     basic_step_r_in_r
-     basic_step_w_in_w
-     basic_step_f_in_f
-     basic_step_rel_eq_rel
-     basic_step_acq_eq_acq
-     basic_step_sc_eq_sc
-     basic_step_r_eq_r
-     basic_step_w_eq_w
-     basic_step_f_eq_f
-     basic_step_fr_eq_fr
-     basic_step_fw_eq_fw
-     basic_step_fracq_eq_fracq
-     basic_step_fwrel_eq_fwrel
-  : same_lab_solveDb.
-
-Lemma basic_step_rel_f_sbE e e' S S'
-      (BSTEP : ESBasicStep.t e e' S S') 
+Lemma store_step_W e e' S S'
+      (BSTEP : basic_step e e' S S')
+      (SSTEP: store_step e e' S S') 
       (wfE: ES.Wf S) :
-  ⦗Rel S'⦘ ⨾ (⦗F S'⦘ ⨾ sb S')^? ⨾ ⦗E S⦘ ≡ 
-  ⦗Rel S ⦘ ⨾ (⦗F S ⦘ ⨾ sb S )^? ⨾ ⦗E S⦘.
-Proof. 
-  arewrite ((⦗F S'⦘ ⨾ sb S')^? ⨾ ⦗E S⦘ ≡ ⦗E S⦘ ⨾ (⦗F S⦘ ⨾ sb S)^?).
-  { rewrite !crE. relsf.
-    apply union_more; auto.
-    rewrite !seqA.
-    rewrite ESBasicStep.basic_step_sbE; eauto.
-    rewrite ES.sbE; auto.
-    arewrite (⦗F S'⦘ ⨾ ⦗E S⦘ ≡ ⦗E S⦘ ⨾ ⦗F S⦘).
-    { rewrite !seq_eqv.
-      apply eqv_rel_more.
-      rewrite set_interC.
-      eapply ESBasicStep.type_step_eq_dom; eauto. }
-    basic_solver. }
-  arewrite (⦗Rel S'⦘ ⨾ ⦗E S⦘ ≡ ⦗Rel S⦘ ⨾ ⦗E S⦘).
-  { rewrite !seq_eqv.
-    apply eqv_rel_more.
-    rewrite set_interC.
-    autorewrite with same_lab_solveDb; eauto.
-    basic_solver. }
-  rewrite ES.sbE; auto.
-  basic_solver 10.
-Qed.
+  E S' ∩₁ W S' ≡₁ E S ∩₁ W S ∪₁ eq e.
+Proof. cdes SSTEP; cdes ACO. step_type_solver. Qed.  
 
-Lemma basic_step_jf_sb_f_acq e e' S S'
-      (BSTEP : ESBasicStep.t e e' S S') 
-      (WF: ES.Wf S) :
-  jf S ⨾ (sb S ⨾ ⦗F S'⦘)^? ⨾ ⦗Acq S'⦘ ≡ jf S ⨾ (sb S ⨾ ⦗F S⦘)^? ⨾ ⦗Acq S⦘.
-Proof. 
-  arewrite (sb S ⨾ ⦗F S'⦘ ≡ sb S ⨾ ⦗F S⦘).
-  { rewrite ES.sbE; auto. rewrite !seqA.
-    arewrite (⦗E S⦘ ⨾ ⦗F S'⦘ ≡ ⦗E S⦘ ⨾ ⦗F S⦘); auto.
-    rewrite !seq_eqv.
-    apply eqv_rel_more.
-    eapply ESBasicStep.type_step_eq_dom; eauto. }
-  assert (jf S ⨾ (sb S ⨾ ⦗F S⦘)^? ≡
-          jf S ⨾ (sb S ⨾ ⦗F S⦘)^? ⨾ ⦗E S⦘) as HH.
-  { split; [|basic_solver 10].
-    rewrite (dom_r WF.(ES.jfE)).
-    rewrite (dom_r WF.(ES.sbE)).
-    basic_solver 20. }
-  seq_rewrite HH. symmetry.
-  seq_rewrite HH. rewrite !seqA.
-  rewrite <- !id_inter.
-  rewrite basic_step_acq_eq_acq with (S':=S'); eauto.
-Qed.
+Lemma store_step_F e e' S S'
+      (BSTEP : basic_step e e' S S')
+      (SSTEP: store_step e e' S S') 
+      (wfE: ES.Wf S) :
+  E S' ∩₁ F S' ≡₁ E S ∩₁ F S.
+Proof. cdes SSTEP; cdes ACO. step_type_solver. Qed.  
+
+Lemma store_step_acq e e' S S'
+      (BSTEP : basic_step e e' S S')
+      (SSTEP: store_step e e' S S') 
+      (wfE: ES.Wf S) :
+  E S' ∩₁ FR S' ∩₁ Acq S' ≡₁ E S ∩₁ FR S ∩₁ Acq S.
+Proof. cdes SSTEP; cdes ACO. step_type_solver. Qed.  
+
+Lemma store_step_Rel e e' S S'
+      (BSTEP : basic_step e e' S S')
+      (SSTEP: store_step e e' S S') 
+      (wfE: ES.Wf S) :
+  E S' ∩₁ FW S' ∩₁ Rel S' ≡₁ E S ∩₁ FW S ∩₁ Rel S ∪₁ eq e ∩₁ Rel S'.
+Proof. cdes SSTEP; cdes ACO. step_type_solver. Qed.  
 
 (******************************************************************************)
-(** ** Step (add_jf) properties *)
+(** ** Update step properties *)
 (******************************************************************************)
 
-Lemma step_add_jf_jf_dom w e e' S S'
-      (BSTEP : ESBasicStep.t e e' S S')
-      (AJF : add_jf w e S S') 
-      (wf : ES.Wf S) : 
-  dom_rel (jf S') ⊆₁ E S.
-Proof. 
-  cdes AJF; cdes BSTEP; cdes BSTEP_.
-  rewrite JF', dom_union. 
-  rewrite wf.(ES.jfE).
-  rewrite step_add_jf_jf_delta_dom; eauto.
-  basic_solver.
-Qed.
+Lemma update_step_E e e' S S'
+      (BSTEP : basic_step e (Some e') S S')
+      (USTEP: update_step e (Some e') S S') :
+  E S' ≡₁ E S ∪₁ eq e ∪₁ eq e'.
+Proof. cdes USTEP. erewrite basic_step_acts_set; eauto. basic_solver. Qed.
 
-Lemma step_add_jf_jfE w e e' S S'
-      (BSTEP : ESBasicStep.t e e' S S') 
-      (AJF : add_jf w e S S') 
-      (wf : ES.Wf S) : 
-  jf S' ⨾ ⦗E S⦘ ≡ jf S.
-Proof.   
-  cdes AJF; cdes BSTEP; cdes BSTEP_.
-  rewrite JF'. 
-  rewrite seq_union_l.
-  rewrite step_add_jf_jf_deltaE; eauto.
-  rewrite ES.jfE; auto. basic_solver 5.
-Qed.
-
-Lemma step_add_jf_jfi lang k k' st st' w e e' S S'
-      (BSTEP_ : ESBasicStep.t_ lang k k' st st' e e' S S') 
-      (AJF : add_jf w e S S') 
-      (wf : ES.Wf S) : 
-  jfi S' ≡ jfi S ∪ jfi_delta S k w e.
-Proof. 
-  cdes AJF; cdes BSTEP_.
-  unfold ES.jfi, jfi_delta.
-  rewrite SB', JF'.
-  rewrite inter_union_l, !inter_union_r.
-  arewrite_false (jf S ∩ ESBasicStep.sb_delta S k e e').
-  { ESBasicStep.step_solver. }
-  arewrite_false (jf_delta w e ∩ sb S). 
-  { ESBasicStep.step_solver. } 
-  relsf.
-  apply union_more; auto.
-  autounfold with ESStepDb.
-  rewrite inter_union_r.
-  arewrite_false (singl_rel w e ∩ (ES.cont_sb_dom S k ∪₁ eq e) × eq_opt e').
-  { ESBasicStep.step_solver. }
-  basic_solver 10.
-Qed.
-
-Lemma step_add_jf_jfe lang k k' st st' w e e' S S'
-      (BSTEP_ : ESBasicStep.t_ lang k k' st st' e e' S S') 
-      (AJF : add_jf w e S S') 
-      (wf : ES.Wf S) : 
-  jfe S' ≡ jfe S ∪ jfe_delta S k w e.
-Proof. 
-  cdes AJF; cdes BSTEP_.
-  unfold ES.jfe, jfe_delta.
-  rewrite SB', JF'.
-  rewrite minus_union_l, !minus_union_r.
-  erewrite minus_disjoint 
-    with (r := jf S) (r' := ESBasicStep.sb_delta S k e e').
-  2 : { split; [|done]. ESBasicStep.step_solver. }
-  erewrite minus_disjoint 
-    with (r := jf_delta w e) (r' := sb S).
-  2 : { split; [|done]. ESBasicStep.step_solver. }
-  apply union_more.
-  { basic_solver. }
-  autounfold with ESStepDb.
-  rewrite !minus_union_r.
-  erewrite minus_disjoint 
-    with (r := singl_rel w e) (r' := (ES.cont_sb_dom S k ∪₁ eq e) × eq_opt e').
-  2 : { split; [|done]. ESBasicStep.step_solver. }
-  rewrite minus_inter_compl.
-  rewrite !interC with (r1 := singl_rel w e).
-  rewrite !interA, !interK.
-  split; [basic_solver|].
-  unfolder. ins. desc.
-  splits; auto. 
-  red. ins. desc. auto.
-Qed.
-
-Lemma step_add_jf_jfi_dom w e e' S S'
-      (BSTEP : ESBasicStep.t e e' S S')
-      (AJF : add_jf w e S S') 
-      (wf : ES.Wf S) : 
-  dom_rel (jfi S') ⊆₁ E S.
-Proof. 
-  unfold ES.jfi.
-  unfolder; ins; desf.
-  eapply step_add_jf_jf_dom; eauto. 
-  basic_solver.
-Qed.
-
-Lemma step_add_jf_jfe_dom w e e' S S'
-      (BSTEP : ESBasicStep.t e e' S S')
-      (AJF : add_jf w e S S') 
-      (wf : ES.Wf S) : 
-  dom_rel (jfe S') ⊆₁ E S.
-Proof. 
-  unfold ES.jfe.
-  unfolder; ins; desf.
-  eapply step_add_jf_jf_dom; eauto. 
-  basic_solver.
-Qed.
-
-Lemma step_add_jf_jfiE w e e' S S'
-      (BSTEP : ESBasicStep.t e e' S S') 
-      (AJF : add_jf w e S S') 
-      (wf : ES.Wf S) : 
-  jfi S' ⨾ ⦗E S⦘ ≡ jfi S.
-Proof.   
-  cdes AJF; cdes BSTEP; cdes BSTEP_.
-  rewrite step_add_jf_jfi; eauto.
-  rewrite seq_union_l.
-  rewrite step_add_jf_jfi_deltaE; eauto.
-  rewrite ES.jfiE; auto. basic_solver 5.
-Qed.
-
-Lemma step_add_jf_jfeE w e e' S S'
-      (BSTEP : ESBasicStep.t e e' S S') 
-      (AJF : add_jf w e S S') 
-      (wf : ES.Wf S) : 
-  jfe S' ⨾ ⦗E S⦘ ≡ jfe S.
-Proof.   
-  cdes AJF; cdes BSTEP; cdes BSTEP_.
-  rewrite step_add_jf_jfe; eauto.
-  rewrite seq_union_l.
-  rewrite step_add_jf_jfe_deltaE; eauto.
-  rewrite ES.jfeE; auto. basic_solver 5.
-Qed.
-
-Lemma step_add_jf_sb_jf lang k k' st st' w e e' S S'
-      (BSTEP_ : ESBasicStep.t_ lang k k' st st' e e' S S') 
-      (AJF : add_jf w e S S') 
+Lemma update_step_R e e' S S'
+      (BSTEP : basic_step e (Some e') S S')
+      (USTEP: update_step e (Some e') S S') 
       (wfE: ES.Wf S) :
-  (sb S' ∪ jf S')＊ ≡ 
-    (sb S ∪ jf S)＊ ⨾ 
-      (ESBasicStep.sb_delta S k e e' ∪ singl_rel w e ∪ eq w × eq_opt e')^?. 
-Proof. 
-  cdes AJF; cdes BSTEP_.
-  assert (ESBasicStep.t e e' S S') as BSTEP.
-  { econstructor. eauto. }
-  autounfold with ESStepDb in *.
-  rewrite SB', JF'. 
-  arewrite 
-    (sb S ∪ ESBasicStep.sb_delta S k e e' ∪ (jf S ∪ singl_rel w e) ≡
-      ESBasicStep.sb_delta S k e e' ∪ singl_rel w e ∪ (sb S ∪ jf S))
-    by basic_solver.
-  erewrite rt_unionE. 
-  apply seq_more; auto.
-  rewrite rt_begin with (r := sb S ∪ jf S).
-  rewrite seq_union_r, seq_id_r. 
-  arewrite_false 
-    ((ESBasicStep.sb_delta S k e e' ∪ singl_rel w e) ⨾ (sb S ∪ jf S)).
-  { ESBasicStep.step_solver. }
-  relsf. 
-  rewrite rtE, crE.
-  apply union_more; auto.
-  (* unroll transitive closure up to 3 iterations *)
-  do 3 rewrite ct_begin, rtE.
-  rewrite !seq_union_r, !seq_id_r.
-  rewrite <- !seqA.
-  arewrite 
-    ((ESBasicStep.sb_delta S k e e' ∪ singl_rel w e)
-     ⨾ (ESBasicStep.sb_delta S k e e' ∪ singl_rel w e) ≡ 
-     ES.cont_sb_dom S k × eq_opt e' ∪ eq w × eq_opt e'). 
-  { unfold ESBasicStep.sb_delta.
-    rewrite !seq_union_l. 
-    arewrite_false 
-      ((ES.cont_sb_dom S k ∪₁ eq e) × eq_opt e'
-      ⨾ (ES.cont_sb_dom S k × eq e ∪ 
-                        (ES.cont_sb_dom S k ∪₁ eq e) × eq_opt e' ∪ singl_rel w e)). 
-    { arewrite (singl_rel w e ⊆ E S × eq e).
-      { basic_solver. }
-      ESBasicStep.step_solver. }
-    rewrite cross_union_r. rewrite !seq_union_r.
-    arewrite_false 
-      (ES.cont_sb_dom S k × eq e ⨾ ES.cont_sb_dom S k × eq_opt e').
-    { ESBasicStep.step_solver. }
-    arewrite_false
-     (ES.cont_sb_dom S k × eq e ⨾ singl_rel w e).
-    { arewrite (singl_rel w e ⊆ E S × eq e).
-      { basic_solver. }
-      ESBasicStep.step_solver. }
-    arewrite_false
-      (singl_rel w e ⨾ ES.cont_sb_dom S k × eq e).
-    { ESBasicStep.step_solver. }
-    arewrite_false
-      (singl_rel w e ⨾ ES.cont_sb_dom S k × eq_opt e').
-    { ESBasicStep.step_solver. }
-    arewrite_false
-      (ES.cont_sb_dom S k × eq e ⨾ ES.cont_sb_dom S k × eq e).
-    { ESBasicStep.step_solver. }
-    arewrite_false
-      (singl_rel w e ⨾ singl_rel w e).
-    { arewrite (singl_rel w e ⊆ E S × eq e).
-      { basic_solver. }
-      ESBasicStep.step_solver. }
-    basic_solver 10. }
-  rewrite <- seqA.
-  arewrite_false 
-    ((ES.cont_sb_dom S k × eq_opt e' ∪ eq w × eq_opt e')
-        ⨾ (ESBasicStep.sb_delta S k e e' ∪ singl_rel w e)).
-  { arewrite (singl_rel w e ⊆ E S × eq e).
-    { basic_solver. }
-    ESBasicStep.step_solver. }
-  unfold ESBasicStep.sb_delta. 
-  basic_solver 10. 
-Qed.
+  E S' ∩₁ R S' ≡₁ E S ∩₁ R S ∪₁ eq e.
+Proof. cdes USTEP; cdes AJF; cdes ACO. step_type_solver. Qed.  
 
-Lemma step_add_jf_sb_jfE w e e' S S'
-      (BSTEP : ESBasicStep.t e e' S S') 
-      (AJF : add_jf w e S S') 
+Lemma update_step_W e e' S S'
+      (BSTEP : basic_step e (Some e') S S')
+      (USTEP: update_step e (Some e') S S') 
       (wfE: ES.Wf S) :
-  (sb S' ∪ jf S')＊ ⨾ ⦗E S⦘ ≡ (sb S ∪ jf S)＊ ⨾ ⦗E S⦘.
-Proof. 
-  cdes AJF; cdes BSTEP; cdes BSTEP_.
-  erewrite step_add_jf_sb_jf; eauto.
-  rewrite crE. relsf.
-  rewrite <- union_false_r with (r := (sb S ∪ jf S)＊ ⨾ ⦗E S⦘) at 2. 
-  apply union_more; auto.
-  split; [|done].
-  ESBasicStep.step_solver.
-Qed.
+  E S' ∩₁ W S' ≡₁ E S ∩₁ W S ∪₁ eq e'.
+Proof. cdes USTEP; cdes AJF; cdes ACO. step_type_solver. Qed.  
 
-Lemma step_add_jf_sb_jf_dom w e e' S S'
-      (BSTEP : ESBasicStep.t e e' S S') 
-      (AJF : add_jf w e S S') 
+Lemma update_step_F e e' S S'
+      (BSTEP : basic_step e (Some e') S S')
+      (USTEP: update_step e (Some e') S S') 
       (wfE: ES.Wf S) :
-  dom_rel ((sb S' ∪ jf S')＊ ⨾ ⦗E S⦘) ⊆₁ E S.
-Proof. 
-  rewrite step_add_jf_sb_jfE; eauto.
-  rewrite rtE, seq_union_l, seq_id_l. 
-  rewrite ES.sbE, ES.jfE; auto.
-  rewrite <- seq_union_r. 
-  rewrite inclusion_ct_seq_eqv_l.
-  basic_solver.
-Qed.
+  E S' ∩₁ F S' ≡₁ E S ∩₁ F S.
+Proof. cdes USTEP; cdes AJF; cdes ACO. step_type_solver. Qed.  
 
-Lemma step_add_jf_cc lang k k' st st' w e e' S S'
-      (BSTEP_ : ESBasicStep.t_ lang k k' st st' e e' S S') 
-      (AJF : add_jf w e S S') 
+Lemma update_step_acq e e' S S'
+      (BSTEP : basic_step e (Some e') S S')
+      (USTEP: update_step e (Some e') S S') 
       (wfE: ES.Wf S) :
-  cc S' ≡ cc S ∪ 
-     cf S' ∩ 
-     (jfe S ⨾ (sb S ∪ jf S)＊ ⨾ 
-          (jfe S ⨾ ESBasicStep.sb_delta S k e e' ∪ jfe_delta S k w e ⨾ (eq e × eq_opt e')^?)).
-Proof. 
-  cdes AJF; cdes BSTEP_.
-  assert (ESBasicStep.t e e' S S') as BSTEP.
-  { econstructor. eauto. }
-  unfold cc at 1. 
-  erewrite dom_rel_helper with (r := jfe S') at 2.
-  2 : eapply step_add_jf_jfe_dom; eauto.
-  rewrite !seqA. 
-  rewrite <- seqA with (r2 := ⦗E S⦘).
-  erewrite dom_rel_helper with (r := (sb S' ∪ jf S')＊ ⨾ ⦗E S⦘).
-  2 : eapply step_add_jf_sb_jf_dom; eauto.
-  rewrite step_add_jf_sb_jfE; eauto.
-  rewrite !seqA. 
-  rewrite <- !seqA with (r2 := ⦗E S⦘).
-  rewrite step_add_jf_jfeE; eauto.
-  rewrite !seqA.
-  rewrite <- !seqA with (r1 := ⦗E S⦘).
-  erewrite <- dom_rel_helper with (r := jfe S').
-  2 : eapply step_add_jf_jfe_dom; eauto.  
-  rewrite SB'. 
-  rewrite step_add_jf_jfe with (S' := S') at 1; eauto.
-  rewrite cr_union_l. relsf.
-  rewrite !inter_union_r.
-  rewrite unionA.
-  apply union_more.
-  { rewrite ESBasicStep.basic_step_cf; eauto. 
-    autounfold with ESStepDb.
-    rewrite <- unionA, !inter_union_l, unionA.
-    rewrite <- union_false_r with (r := cc S).
-    apply union_more.
-    { by unfold cc. }
-    split; [|done].
-    ESBasicStep.step_solver. }
-  rewrite unionC, unionA.
-  apply union_more; auto.
-  rewrite !crE. relsf.
-  arewrite_false (jfe_delta S k w e ⨾ sb S). 
-  { autounfold with ESStepDb. 
-    arewrite (singl_rel w e ⊆ E S × eq e).
-    { basic_solver. }
-    ESBasicStep.step_solver. }
-  relsf.
-  rewrite !inter_union_r.
-  rewrite unionC.
-  apply union_more; auto.
-  apply inter_rel_more; auto.  
-  do 2 (apply seq_more; auto).  
-  autounfold with ESStepDb. 
-  rewrite cross_union_r.
-  relsf. rewrite !seqA.
-  arewrite_false (singl_rel w e ⨾ ES.cont_sb_dom S k × eq e).
-  { arewrite (singl_rel w e ⊆ E S × eq e).
-    { basic_solver. }
-    ESBasicStep.step_solver. }
-  arewrite_false (singl_rel w e ⨾ ES.cont_sb_dom S k × eq_opt e').
-  { arewrite (singl_rel w e ⊆ E S × eq e).
-    { basic_solver. }
-    ESBasicStep.step_solver. }
-  basic_solver 10.
-Qed.  
+  E S' ∩₁ FR S' ∩₁ Acq S' ≡₁ E S ∩₁ FR S ∩₁ Acq S ∪₁ eq e ∩₁ Acq S'.
+Proof. cdes USTEP; cdes AJF; cdes ACO. step_type_solver. Qed.  
 
-Lemma step_add_jf_ccE w e e' S S'
-      (BSTEP : ESBasicStep.t e e' S S') 
-      (AJF : add_jf w e S S') 
+Lemma update_step_Rel e e' S S'
+      (BSTEP : basic_step e (Some e') S S')
+      (USTEP: update_step e (Some e') S S') 
       (wfE: ES.Wf S) :
-  cc S' ⨾ ⦗E S⦘ ≡ cc S.
-Proof. 
-  cdes AJF; cdes BSTEP; cdes BSTEP_.
-  rewrite step_add_jf_cc; eauto.
-  rewrite seq_union_l.
-  rewrite interC.
-  rewrite <- lib.AuxRel.seq_eqv_inter_lr.
-  rewrite !seqA, seq_union_l.
-  rewrite !seqA.
-  arewrite_false 
-    (ESBasicStep.sb_delta S k e e' ⨾ ⦗E S⦘).
-  { ESBasicStep.step_solver. }
-  arewrite_false
-   (jfe_delta S k w e ⨾ (eq e × eq_opt e')^? ⨾ ⦗E S⦘).
-  { autounfold with ESStepDb. 
-    arewrite (singl_rel w e ⊆ E S × eq e).
-    { basic_solver. }
-    ESBasicStep.step_solver. }
-  relsf.
-  rewrite ccE. basic_solver.
-Qed.
-
-Lemma step_add_jf_jf_rmw w e e' S S'
-      (BSTEP : ESBasicStep.t e e' S S') 
-      (AJF : add_jf w e S S') 
-      (wfE: ES.Wf S) :
-  jf S' ⨾ rmw S' ≡ jf S ⨾ rmw S ∪ eq w × eq_opt e'.
-Proof. 
-  cdes AJF; cdes BSTEP; cdes BSTEP_.
-  rewrite JF', RMW'.
-  relsf. rewrite unionA.
-  apply union_more; auto.
-  arewrite_false (jf_delta w e ⨾ rmw S).
-  { ESBasicStep.step_solver. }
-  arewrite_false (jf S ⨾ ESBasicStep.rmw_delta e e').
-  { ESBasicStep.step_solver. }
-  autounfold with ESStepDb.
-  basic_solver 10.
-Qed.  
-
-Lemma step_add_jf_jf_rmwE w e e' S S'
-      (BSTEP : ESBasicStep.t e e' S S') 
-      (AJF : add_jf w e S S') 
-      (wfE: ES.Wf S) :
-  jf S' ⨾ rmw S' ⨾ ⦗E S⦘ ≡ jf S ⨾ rmw S.
-Proof. 
-  cdes AJF; cdes BSTEP; cdes BSTEP_.
-  rewrite <- seqA.
-  rewrite step_add_jf_jf_rmw; eauto.
-  relsf.
-  arewrite_false (eq w × eq_opt e' ⨾ ⦗E S⦘).
-  { ESBasicStep.step_solver. }
-  rewrite ES.rmwE; auto. basic_solver 10.
-Qed.
-
-Lemma step_add_jf_rsE w e e' S S'
-      (BSTEP : ESBasicStep.t e e' S S') 
-      (AJF : add_jf w e S S') 
-      (wfE: ES.Wf S) :
-  rs S' ⨾ ⦗E S⦘ ≡ rs S ⨾ ⦗E S⦘.
-Proof. 
-  cdes AJF; cdes BSTEP; cdes BSTEP_.
-  unfold rs at 1. rewrite !seqA.
-  arewrite ((jf S' ⨾ rmw S')＊ ⨾ ⦗E S⦘ ≡ (jf S ⨾ rmw S)＊ ⨾ ⦗E S⦘).
-  { rewrite !rtE. relsf.
-    eapply union_more; auto.
-    split. 
-    { rewrite !seq_eqv_r.
-      intros x y [TC Ey].
-      split; auto.
-      induction TC. 
-      { eapply t_step.
-        eapply step_add_jf_jf_rmwE; eauto.
-        unfolder in *. desc. eauto. }
-      eapply t_trans; eauto.
-      eapply IHTC1.
-      eapply step_add_jf_jf_dom; eauto.
-      apply ct_begin in TC2.
-      generalize TC2. basic_solver 10. }
-    apply seq_mori; [|done].
-    apply clos_trans_mori. 
-    rewrite step_add_jf_jf_rmw with (S' := S'); eauto.
-    basic_solver. }
-  arewrite ((jf S ⨾ rmw S)＊ ⨾ ⦗E S⦘ ≡ ⦗E S⦘ ⨾ (jf S ⨾ rmw S)＊ ⨾ ⦗E S⦘).
-  { rewrite rtE. relsf.
-    apply union_more; auto.
-    rewrite restr_clos_trans_eq with (s := E S).
-    2 : { rewrite ES.jfE, ES.rmwE; auto. basic_solver 10. }
-    basic_solver. }
-  seq_rewrite basic_step_w_sb_loc_wE; eauto.
-  unfold rs.
-  rewrite !seqA.
-  basic_solver.
-Qed.
-
-Lemma step_add_jf_releaseE w e e' S S'
-      (BSTEP : ESBasicStep.t e e' S S') 
-      (AJF : add_jf w e S S') 
-      (wfE: ES.Wf S) :
-  release S' ⨾ ⦗E S⦘ ≡ release S ⨾ ⦗E S⦘.
-Proof. 
-  unfold release at 1.
-  rewrite !seqA.
-  arewrite (rs S' ⨾ ⦗E S⦘ ≡ ⦗E S⦘ ⨾ rs S ⨾ ⦗E S⦘).
-  { rewrite step_add_jf_rsE; eauto.
-    rewrite rsE; auto.
-    basic_solver. }
-  seq_rewrite basic_step_rel_f_sbE; eauto. 
-  unfold release.
-  rewrite ES.sbE, rsE; auto.
-  basic_solver 20.
-Qed.
-
-Lemma step_add_jf_sw lang k k' st st' w e e' S S'
-      (BSTEP_ : ESBasicStep.t_ lang k k' st st' e e' S S') 
-      (AJF : add_jf w e S S') 
-      (nF' : eq_opt e' ∩₁ F S' ⊆₁ ∅)
-      (wfE: ES.Wf S) :
-  sw S' ≡ sw S ∪ sw_delta S S' k e e'. 
-Proof. 
-  cdes AJF; cdes BSTEP_.
-  assert (ESBasicStep.t e e' S S') as BSTEP.
-  { econstructor. eauto. }
-  unfold sw_delta.
-  unfold sw at 1.
-  erewrite dom_rel_helper with (r := jf S').
-  2 : eapply step_add_jf_jf_dom; eauto.
-  rewrite !seqA, <- seqA.
-  rewrite step_add_jf_releaseE; eauto.
-  rewrite !seqA.
-  rewrite <- seqA with (r1 := ⦗E S⦘).
-  erewrite <- dom_rel_helper with (r := jf S').
-  2 : eapply step_add_jf_jf_dom; eauto.
-  rewrite SB', JF'.
-  rewrite seq_union_l, cr_union_l.
-  relsf. rewrite unionA.
-  apply union_more.
-  { rewrite basic_step_jf_sb_f_acq; eauto. }
-  rewrite crE. relsf.
-  rewrite !seqA.
-  arewrite_false (ESBasicStep.sb_delta S k e e' ⨾ ⦗F S'⦘).
-  { unfold ESBasicStep.sb_delta.
-    clear -nF' rR'.
-    rewrite seq_union_l, <- !cross_inter_r.
-    arewrite (eq e ∩₁ F S' ⊆₁ ∅).
-    { type_solver. }
-    rewrite nF'.
-    basic_solver. }
-  arewrite_false (jf_delta w e ⨾ sb S).
-  { ESBasicStep.step_solver. }
-  arewrite_false (jf S ⨾ ⦗eq e⦘).
-  { ESBasicStep.step_solver. }
-  unfold jf_delta.
-  basic_solver 10.
-Qed.  
-
-Lemma step_add_jf_sw_dom lang k k' st st' w e e' S S'
-      (BSTEP_ : ESBasicStep.t_ lang k k' st st' e e' S S') 
-      (AJF : add_jf w e S S') 
-      (nF' : eq_opt e' ∩₁ F S' ⊆₁ ∅)
-      (wfE: ES.Wf S) :
-  dom_rel (sw S') ⊆₁ E S.
-Proof. 
-  cdes AJF; cdes BSTEP_.
-  rewrite step_add_jf_sw; eauto.
-  ESBasicStep.step_solver.
-Qed.
-
-Lemma step_add_jf_swE w e e' S S' 
-      (BSTEP : ESBasicStep.t e e' S S') 
-      (AJF : add_jf w e S S') 
-      (nF' : eq_opt e' ∩₁ F S' ⊆₁ ∅)
-      (wfE: ES.Wf S) :
-  sw S' ⨾ ⦗E S⦘ ≡ sw S.
-Proof. 
-  cdes AJF; cdes BSTEP; cdes BSTEP_.
-  rewrite step_add_jf_sw; eauto.
-  relsf. rewrite basic_step_sw_deltaE; eauto.
-  rewrite swE; auto. basic_solver 5.
-Qed.
-
-Lemma step_add_jf_hb lang k k' st st' w e e' S S' 
-      (BSTEP_ : ESBasicStep.t_ lang k k' st st' e e' S S') 
-      (AJF : add_jf w e S S') 
-      (nF' : eq_opt e' ∩₁ F S' ⊆₁ ∅)
-      (wfE: ES.Wf S) :
-  hb S' ≡ hb S ∪ hb_delta S S' k e e'.
-Proof.
-  cdes AJF; cdes BSTEP_.
-  assert (ESBasicStep.t e e' S S') as BSTEP.
-  { subst. econstructor. eauto. }
-  unfold hb at 1.
-  rewrite SB'. 
-  rewrite step_add_jf_sw; eauto.
-  arewrite 
-    (sb S ∪ ESBasicStep.sb_delta S k e e' ∪ (sw S ∪ sw_delta S S' k e e') ≡
-     (ESBasicStep.sb_delta S k e e' ∪ sw_delta S S' k e e') ∪ (sb S ∪ sw S))
-    by basic_solver.
-  rewrite ct_unionE.
-  unfold hb. 
-  apply union_more; auto.
-  rewrite <- cr_of_ct.
-  rewrite basic_step_hb_delta_alt; eauto.
-Qed.
-
-Lemma step_add_jf_hb_dom w e e' S S' 
-      (BSTEP : ESBasicStep.t e e' S S') 
-      (AJF : add_jf w e S S') 
-      (nF' : eq_opt e' ∩₁ F S' ⊆₁ ∅)
-      (wfE: ES.Wf S) :
-  dom_rel (hb S') ⊆₁ E S ∪₁ eq e.
-Proof. 
-  cdes AJF; cdes BSTEP; cdes BSTEP_.
-  rewrite step_add_jf_hb; eauto.
-  rewrite dom_union.
-  rewrite basic_step_hb_delta_dom; eauto.
-  rewrite hbE; auto.
-  basic_solver.
-Qed. 
-
-Lemma step_add_jf_hbE w e e' S S' 
-      (BSTEP : ESBasicStep.t e e' S S') 
-      (AJF : add_jf w e S S') 
-      (nF' : eq_opt e' ∩₁ F S' ⊆₁ ∅)
-      (wfE: ES.Wf S) :
-  hb S' ⨾ ⦗E S⦘ ≡ hb S.
-Proof. 
-  cdes AJF; cdes BSTEP; cdes BSTEP_.
-  rewrite step_add_jf_hb; eauto.
-  relsf.
-  rewrite basic_step_hb_deltaE; eauto.
-  rewrite hbE; auto. basic_solver 5.
-Qed. 
+  E S' ∩₁ FW S' ∩₁ Rel S' ≡₁ E S ∩₁ FW S ∩₁ Rel S ∪₁ (eq e' ∩₁ Rel S').
+Proof. cdes USTEP; cdes AJF; cdes ACO. step_type_solver. Qed.  
 
 (******************************************************************************)
 (** ** Step (same jf) properties *)
 (******************************************************************************)
 
 Lemma step_same_jf_jfi e e' S S'
-      (BSTEP : ESBasicStep.t e e' S S') 
+      (BSTEP : basic_step e e' S S') 
       (JF' : jf S' ≡ jf S) 
       (wf : ES.Wf S) : 
   jfi S' ≡ jfi S.
@@ -1620,13 +319,13 @@ Proof.
   unfold ES.jfi.
   rewrite SB', JF'.
   rewrite inter_union_r.
-  arewrite_false (jf S ∩ ESBasicStep.sb_delta S k e e').
-  { ESBasicStep.step_solver. }
+  arewrite_false (jf S ∩ sb_delta S k e e').
+  { step_solver. }
   basic_solver.
 Qed.
 
 Lemma step_same_jf_jfe e e' S S'
-      (BSTEP : ESBasicStep.t e e' S S') 
+      (BSTEP : basic_step e e' S S') 
       (JF' : jf S' ≡ jf S) 
       (wf : ES.Wf S) : 
   jfe S' ≡ jfe S.
@@ -1635,33 +334,33 @@ Proof.
   unfold ES.jfe.
   rewrite SB', JF'.
   rewrite minus_union_r.
-  rewrite minus_disjoint with (r' := ESBasicStep.sb_delta S k e e').
-  2 : { split; [|done]. ESBasicStep.step_solver. }
+  rewrite minus_disjoint with (r' := sb_delta S k e e').
+  2 : { split; [|done]. step_solver. }
   basic_solver.
 Qed.
 
 Lemma step_same_jf_sb_jf lang k k' st st' e e' S S'
-      (BSTEP_ : ESBasicStep.t_ lang k k' st st' e e' S S') 
+      (BSTEP_ : basic_step_ lang k k' st st' e e' S S') 
       (JF' : jf S' ≡ jf S) 
       (wf : ES.Wf S) : 
   (sb S' ∪ jf S')＊ ≡ 
-    (sb S ∪ jf S)＊ ⨾ (ESBasicStep.sb_delta S k e e')^?. 
+    (sb S ∪ jf S)＊ ⨾ (sb_delta S k e e')^?. 
 Proof. 
   cdes BSTEP_.
-  assert (ESBasicStep.t e e' S S') as BSTEP.
+  assert (basic_step e e' S S') as BSTEP.
   { econstructor. eauto. }
   rewrite SB', JF'. 
   arewrite 
-    (sb S ∪ ESBasicStep.sb_delta S k e e' ∪ jf S ≡
-      ESBasicStep.sb_delta S k e e' ∪ (sb S ∪ jf S))
+    (sb S ∪ sb_delta S k e e' ∪ jf S ≡
+      sb_delta S k e e' ∪ (sb S ∪ jf S))
     by basic_solver.
   erewrite rt_unionE. 
   apply seq_more; auto.
   rewrite rt_begin with (r := sb S ∪ jf S).
   rewrite seq_union_r, seq_id_r. 
   arewrite_false 
-    (ESBasicStep.sb_delta S k e e' ⨾ (sb S ∪ jf S)).
-  { ESBasicStep.step_solver. }
+    (sb_delta S k e e' ⨾ (sb S ∪ jf S)).
+  { step_solver. }
   relsf. 
   rewrite rtE, crE.
   apply union_more; auto.
@@ -1670,34 +369,34 @@ Proof.
   rewrite !seq_union_r, !seq_id_r.
   rewrite <- !seqA.
   arewrite 
-    ((ESBasicStep.sb_delta S k e e')
-     ⨾ (ESBasicStep.sb_delta S k e e') ≡ 
+    ((sb_delta S k e e')
+     ⨾ (sb_delta S k e e') ≡ 
      ES.cont_sb_dom S k × eq_opt e'). 
-  { unfold ESBasicStep.sb_delta.
+  { unfold sb_delta.
     rewrite !seq_union_l. 
     arewrite_false 
       ((ES.cont_sb_dom S k ∪₁ eq e) × eq_opt e'
       ⨾ (ES.cont_sb_dom S k × eq e ∪ 
                         (ES.cont_sb_dom S k ∪₁ eq e) × eq_opt e')). 
-    { unfold eq_opt, opt_ext in *. ESBasicStep.step_solver. }
+    { unfold eq_opt, opt_ext in *. step_solver. }
     rewrite cross_union_r. rewrite !seq_union_r.
     arewrite_false 
       (ES.cont_sb_dom S k × eq e ⨾ ES.cont_sb_dom S k × eq_opt e').
-    { ESBasicStep.step_solver. }
+    { step_solver. }
     arewrite_false
       (ES.cont_sb_dom S k × eq e ⨾ ES.cont_sb_dom S k × eq e).
-    { ESBasicStep.step_solver. }
+    { step_solver. }
     basic_solver 10. }
   rewrite <- seqA.
   arewrite_false 
-    ((ES.cont_sb_dom S k × eq_opt e') ⨾ (ESBasicStep.sb_delta S k e e')).
-  { ESBasicStep.step_solver. }
-  unfold ESBasicStep.sb_delta. 
+    ((ES.cont_sb_dom S k × eq_opt e') ⨾ (sb_delta S k e e')).
+  { step_solver. }
+  unfold sb_delta. 
   basic_solver 10. 
 Qed.
 
 Lemma step_same_jf_sb_jfE e e' S S'
-      (BSTEP : ESBasicStep.t e e' S S') 
+      (BSTEP : basic_step e e' S S') 
       (JF' : jf S' ≡ jf S) 
       (wfE: ES.Wf S) :
   (sb S' ∪ jf S')＊ ⨾ ⦗E S⦘ ≡ (sb S ∪ jf S)＊ ⨾ ⦗E S⦘.
@@ -1708,18 +407,18 @@ Proof.
   rewrite <- union_false_r with (r := (sb S ∪ jf S)＊ ⨾ ⦗E S⦘) at 2. 
   apply union_more; auto.
   split; [|done].
-  ESBasicStep.step_solver.
+  step_solver.
 Qed.
 
 Lemma step_same_jf_cc lang k k' st st' e e' S S'
-      (BSTEP_ : ESBasicStep.t_ lang k k' st st' e e' S S') 
+      (BSTEP_ : basic_step_ lang k k' st st' e e' S S') 
       (JF' : jf S' ≡ jf S) 
       (wfE: ES.Wf S) :
   cc S' ≡ cc S ∪ 
-     cf S' ∩  (jfe S ⨾ (sb S ∪ jf S)＊ ⨾ (jfe S ⨾ ESBasicStep.sb_delta S k e e')).
+     cf S' ∩  (jfe S ⨾ (sb S ∪ jf S)＊ ⨾ (jfe S ⨾ sb_delta S k e e')).
 Proof. 
   cdes BSTEP_.
-  assert (ESBasicStep.t e e' S S') as BSTEP.
+  assert (basic_step e e' S S') as BSTEP.
   { econstructor. eauto. }
   unfold cc at 1. 
   rewrite step_same_jf_jfe; eauto.
@@ -1736,18 +435,18 @@ Proof.
   rewrite cr_union_l. relsf.
   rewrite !inter_union_r.
   apply union_more; auto.
-  rewrite ESBasicStep.basic_step_cf; eauto. 
+  rewrite basic_step_cf; eauto. 
   autounfold with ESStepDb.
   rewrite <- unionA, !inter_union_l, unionA.
   rewrite <- union_false_r with (r := cc S).
   apply union_more.
   { by unfold cc. }
   split; [|done].
-  ESBasicStep.step_solver. 
+  step_solver. 
 Qed.
 
 Lemma step_same_jf_ccE e e' S S'
-      (BSTEP : ESBasicStep.t e e' S S') 
+      (BSTEP : basic_step e e' S S') 
       (JF' : jf S' ≡ jf S) 
       (wfE: ES.Wf S) :
   cc S' ⨾ ⦗E S⦘ ≡ cc S.
@@ -1759,14 +458,14 @@ Proof.
   rewrite <- lib.AuxRel.seq_eqv_inter_lr.
   rewrite !seqA.
   arewrite_false 
-    (ESBasicStep.sb_delta S k e e' ⨾ ⦗E S⦘).
-  { ESBasicStep.step_solver. }
+    (sb_delta S k e e' ⨾ ⦗E S⦘).
+  { step_solver. }
   relsf.
   rewrite ccE. basic_solver.
 Qed.
 
 Lemma step_same_jf_rsE e e' S S'
-      (BSTEP : ESBasicStep.t e e' S S') 
+      (BSTEP : basic_step e e' S S') 
       (JF' : jf S' ≡ jf S) 
       (RMW' : rmw S' ≡ rmw S) 
       (wfE: ES.Wf S) :
@@ -1788,7 +487,7 @@ Proof.
 Qed.
 
 Lemma step_same_jf_releaseE e e' S S'
-      (BSTEP : ESBasicStep.t e e' S S') 
+      (BSTEP : basic_step e e' S S') 
       (JF' : jf S' ≡ jf S) 
       (RMW' : rmw S' ≡ rmw S) 
       (wfE: ES.Wf S) :
@@ -1807,14 +506,14 @@ Proof.
 Qed.
 
 Lemma step_same_jf_sw lang k k' st st' e e' S S'
-      (BSTEP_ : ESBasicStep.t_ lang k k' st st' e e' S S') 
+      (BSTEP_ : basic_step_ lang k k' st st' e e' S S') 
       (JF' : jf S' ≡ jf S) 
       (RMW' : rmw S' ≡ rmw S) 
       (wfE: ES.Wf S) :
   sw S' ≡ sw S ∪ sw_delta S S' k e e'.
 Proof. 
   cdes BSTEP_.
-  assert (ESBasicStep.t e e' S S') as BSTEP.
+  assert (basic_step e e' S S') as BSTEP.
   { econstructor. eauto. }
   unfold sw at 1.
   rewrite JF'. 
@@ -1830,26 +529,26 @@ Proof.
   unfold sw_delta.
   rewrite JF'.
   arewrite_false (jf S ⨾ ⦗eq e⦘).
-  { ESBasicStep.step_solver. }
+  { step_solver. }
   basic_solver 10.
 Qed.  
 
 Lemma step_same_jf_hb lang k k' st st' e e' S S'
-      (BSTEP_ : ESBasicStep.t_ lang k k' st st' e e' S S') 
+      (BSTEP_ : basic_step_ lang k k' st st' e e' S S') 
       (JF' : jf S' ≡ jf S) 
       (RMW' : rmw S' ≡ rmw S) 
       (wfE: ES.Wf S) :
   hb S' ≡ hb S ∪ hb_delta S S' k e e'.
 Proof.
   cdes BSTEP_.
-  assert (ESBasicStep.t e e' S S') as BSTEP.
+  assert (basic_step e e' S S') as BSTEP.
   { subst. econstructor. eauto. }
   unfold hb at 1.
   rewrite SB'. 
   rewrite step_same_jf_sw; eauto.
   arewrite 
-    (sb S ∪ ESBasicStep.sb_delta S k e e' ∪ (sw S ∪ sw_delta S S' k e e') ≡
-     (ESBasicStep.sb_delta S k e e' ∪ sw_delta S S' k e e') ∪ (sb S ∪ sw S))
+    (sb S ∪ sb_delta S k e e' ∪ (sw S ∪ sw_delta S S' k e e') ≡
+     (sb_delta S k e e' ∪ sw_delta S S' k e e') ∪ (sb S ∪ sw S))
     by basic_solver.
   rewrite ct_unionE.
   unfold hb. 
@@ -1859,7 +558,7 @@ Proof.
 Qed.
 
 Lemma step_same_jf_hb_dom e e' S S' 
-      (BSTEP : ESBasicStep.t e e' S S') 
+      (BSTEP : basic_step e e' S S') 
       (JF' : jf S' ≡ jf S) 
       (RMW' : rmw S' ≡ rmw S) 
       (wfE: ES.Wf S) :
@@ -1874,7 +573,7 @@ Proof.
 Qed. 
 
 Lemma step_same_jf_hbE e e' S S' 
-      (BSTEP : ESBasicStep.t e e' S S') 
+      (BSTEP : basic_step e e' S S') 
       (JF' : jf S' ≡ jf S) 
       (RMW' : rmw S' ≡ rmw S) 
       (wfE: ES.Wf S) :
@@ -1888,7 +587,7 @@ Proof.
 Qed. 
 
 Lemma step_same_jf_ecf_restr e e' S S'
-      (BSTEP : ESBasicStep.t e e' S S') 
+      (BSTEP : basic_step e e' S S') 
       (JF' : jf S' ≡ jf S) 
       (RMW' : rmw S' ≡ rmw S) 
       (wfE: ES.Wf S) :
@@ -1899,7 +598,7 @@ Proof.
   rewrite !crE. relsf.
   rewrite !restr_union.
   repeat apply union_more.
-  { eapply ESBasicStep.basic_step_cf_restr; eauto. }
+  { eapply basic_step_cf_restr; eauto. }
   { rewrite restr_relE, !seqA.
     arewrite (⦗E S⦘ ⨾ (hb S')⁻¹ ≡ (hb S)⁻¹ ⨾ ⦗E S⦘).
     { rewrite <- transp_eqv_rel, <- transp_seq.
@@ -1907,13 +606,13 @@ Proof.
       rewrite hbE; auto.
       basic_solver 10. }
     rewrite <- restr_relE.
-    rewrite ESBasicStep.basic_step_cf_restr; eauto. }
+    rewrite basic_step_cf_restr; eauto. }
   { rewrite restr_relE, !seqA.
     rewrite step_same_jf_hbE; eauto.
     rewrite hbE; auto.
     arewrite (⦗E S⦘ ⨾ cf S' ⨾ ⦗E S⦘ ≡ cf S).
     { rewrite <- restr_relE.
-      rewrite ESBasicStep.basic_step_cf_restr; eauto. }
+      rewrite basic_step_cf_restr; eauto. }
     rewrite hbE; auto.
     basic_solver 10. }
   rewrite restr_relE, !seqA.
@@ -1928,12 +627,12 @@ Proof.
     basic_solver 10. }
   arewrite (⦗E S⦘ ⨾ cf S' ⨾ ⦗E S⦘ ≡ cf S).
   { rewrite <- restr_relE.
-    rewrite ESBasicStep.basic_step_cf_restr; eauto. }
+    rewrite basic_step_cf_restr; eauto. }
   done.
 Qed.
 
 Lemma step_same_jf_jf_necf e e' S S'
-      (BSTEP_ : ESBasicStep.t e e' S S') 
+      (BSTEP_ : basic_step e e' S S') 
       (JF' : jf S' ≡ jf S) 
       (RMW' : rmw S' ≡ rmw S) 
       (wfE: ES.Wf S) 
@@ -1952,36 +651,32 @@ Proof.
 Qed.
 
 (******************************************************************************)
-(** ** Step (add_co) properties *)
-(******************************************************************************)
-
-
-(******************************************************************************)
 (** ** Step properties *)
 (******************************************************************************)
 
 Lemma step_ew_mon e e' S S'
-      (STEP : t_ e e' S S') :
+      (STEP : step_ e e' S S') :
   ew S ⊆ ew S'.
 Proof. 
-  unfold t_, t_fence, t_load, t_store, t_update in STEP. 
-  desf; try cdes AEW; generalize EW'; basic_solver.
+  unfold_step_ STEP;
+  desf; try cdes AEW; 
+  generalize EW'; basic_solver.
 Qed.  
 
 Lemma step_ccE e e' S S'
-      (BSTEP : ESBasicStep.t e e' S S') 
-      (STEP : t_ e e' S S') 
+      (BSTEP : basic_step e e' S S') 
+      (STEP : step_ e e' S S') 
       (wfE: ES.Wf S) :
   cc S' ⨾ ⦗E S⦘ ≡ cc S.
 Proof. 
   cdes BSTEP; cdes BSTEP_.
-  unfold t_, t_fence, t_load, t_store, t_update in STEP. 
-  desf; eauto using step_add_jf_ccE, step_same_jf_ccE.
+  unfold_step_ STEP;
+  desf; eauto using add_jf_ccE, step_same_jf_ccE.
 Qed.
 
 Lemma step_vis_mon e e' S S'
-      (BSTEP : ESBasicStep.t e e' S S') 
-      (STEP : t_ e e' S S')
+      (BSTEP : basic_step e e' S S') 
+      (STEP : step_ e e' S S')
       (wfE: ES.Wf S) :
   vis S ⊆₁ vis S'. 
 Proof. 
@@ -1989,7 +684,7 @@ Proof.
   unfold vis. 
   intros x VIS.
   splits; desf.
-  { eapply ESBasicStep.basic_step_acts_set_mon; eauto. }
+  { eapply basic_step_acts_set_mon; eauto. }
   arewrite (eq x ⊆₁ E S ∩₁ eq x) by basic_solver.
   rewrite <- seq_eqv.
   rewrite <- seqA.
@@ -1998,32 +693,33 @@ Proof.
   apply seq_mori.
   { eapply step_ew_mon; eauto. }
   apply clos_refl_sym_mori.
-  eapply ESBasicStep.basic_step_sb_mon; eauto.
+  eapply basic_step_sb_mon; eauto.
 Qed.
 
 Lemma step_hb lang k k' st st' e e' S S'
-      (BSTEP_ : ESBasicStep.t_ lang k k' st st' e e' S S') 
-      (STEP : t_ e e' S S')
+      (BSTEP_ : basic_step_ lang k k' st st' e e' S S') 
+      (STEP : step_ e e' S S')
       (wfE: ES.Wf S) :
   hb S' ≡ hb S ∪ hb_delta S S' k e e'.
 Proof. 
   cdes BSTEP_.
-  assert (ESBasicStep.rmw_delta e None ≡ ∅₂) as RMW_None.
-  { split; [|done]. ESBasicStep.step_solver. }
-  unfold t_, t_fence, t_load, t_store, t_update in STEP; desf.
+  assert (rmw_delta e None ≡ ∅₂) as RMW_None.
+  { split; [|done]. step_solver. }
+  unfold_step_ STEP.
   all : try by (
     erewrite step_same_jf_hb; eauto;
-    rewrite RMW', RMW_None; 
+    rewrite RMW', nUPD; 
+    unfold rmw_delta;
     basic_solver
   ).
-  all : rewrite step_add_jf_hb; eauto.
+  all : rewrite add_jf_hb; eauto.
   { basic_solver. }
   cdes AEW. type_solver.
 Qed.
 
 Lemma step_hb_dom e e' S S' 
-      (BSTEP : ESBasicStep.t e e' S S') 
-      (STEP : t_ e e' S S')
+      (BSTEP : basic_step e e' S S') 
+      (STEP : step_ e e' S S')
       (wfE: ES.Wf S) :
   dom_rel (hb S') ⊆₁ E S ∪₁ eq e.
 Proof. 
@@ -2036,8 +732,8 @@ Proof.
 Qed. 
 
 Lemma step_hbE e e' S S' 
-      (BSTEP : ESBasicStep.t e e' S S') 
-      (STEP : t_ e e' S S')
+      (BSTEP : basic_step e e' S S') 
+      (STEP : step_ e e' S S')
       (wfE: ES.Wf S) :
   hb S' ⨾ ⦗E S⦘ ≡ hb S.
 Proof. 
@@ -2047,196 +743,3 @@ Proof.
   rewrite basic_step_hb_deltaE; eauto.
   rewrite hbE; auto. basic_solver 5.
 Qed. 
-
-(******************************************************************************)
-(** ** Tactic for load/store/fence/update R/W/F lemmas *)
-(******************************************************************************)
-
-Ltac step_type_solver :=
-  erewrite ESBasicStep.basic_step_acts_set; eauto;
-  unfold eq_opt;
-  rewrite !set_inter_union_l;
-  autorewrite with same_lab_solveDb; 
-  eauto; type_solver 10.
-  
-(******************************************************************************)
-(** ** Fence step properties *)
-(******************************************************************************)
-
-Lemma fence_step_E e e' S S'
-      (BSTEP : ESBasicStep.t e e' S S')
-      (FSTEP: t_fence e e' S S') :
-  E S' ≡₁ E S ∪₁ eq e.
-Proof. cdes FSTEP. subst. by apply ESBasicStep.basic_step_nupd_acts_set. Qed.
-
-Lemma fence_step_R e e' S S'
-      (BSTEP : ESBasicStep.t e e' S S')
-      (FSTEP: t_fence e e' S S') 
-      (wfE: ES.Wf S) :
-  E S' ∩₁ R S' ≡₁ E S ∩₁ R S.
-Proof. cdes FSTEP. step_type_solver. Qed.  
-
-Lemma fence_step_W e e' S S'
-      (BSTEP : ESBasicStep.t e e' S S')
-      (FSTEP: t_fence e e' S S') 
-      (wfE: ES.Wf S) :
-  E S' ∩₁ W S' ≡₁ E S ∩₁ W S.
-Proof. cdes FSTEP. step_type_solver. Qed.  
-
-Lemma fence_step_F e e' S S'
-      (BSTEP : ESBasicStep.t e e' S S')
-      (FSTEP: t_fence e e' S S') 
-      (wfE: ES.Wf S) :
-  E S' ∩₁ F S' ≡₁ E S ∩₁ F S ∪₁ eq e.
-Proof. cdes FSTEP. step_type_solver. Qed.  
-
-Lemma fence_step_acq e e' S S'
-      (BSTEP : ESBasicStep.t e e' S S')
-      (FSTEP: t_fence e e' S S') 
-      (wfE: ES.Wf S) :
-  E S' ∩₁ FR S' ∩₁ Acq S' ≡₁ E S ∩₁ FR S ∩₁ Acq S ∪₁ eq e ∩₁ Acq S'.
-Proof. cdes FSTEP. step_type_solver. Qed.  
-
-Lemma fence_step_Rel e e' S S'
-      (BSTEP : ESBasicStep.t e e' S S')
-      (FSTEP: t_fence e e' S S') 
-      (wfE: ES.Wf S) :
-  E S' ∩₁ FW S' ∩₁ Rel S' ≡₁ E S ∩₁ FW S ∩₁ Rel S ∪₁ eq e ∩₁ Rel S'.
-Proof. cdes FSTEP. step_type_solver. Qed.  
-
-(******************************************************************************)
-(** ** Load step properties *)
-(******************************************************************************)
-
-Lemma load_step_E e e' S S'
-      (BSTEP : ESBasicStep.t e e' S S')
-      (LSTEP: t_load e e' S S') :
-  E S' ≡₁ E S ∪₁ eq e.
-Proof. cdes LSTEP. subst. by apply ESBasicStep.basic_step_nupd_acts_set. Qed.
-
-Lemma load_step_R e e' S S'
-      (BSTEP : ESBasicStep.t e e' S S')
-      (LSTEP: t_load e e' S S') 
-      (wfE: ES.Wf S) :
-  E S' ∩₁ R S' ≡₁ E S ∩₁ R S ∪₁ eq e.
-Proof. cdes LSTEP; cdes AJF. step_type_solver. Qed.  
-
-Lemma load_step_W e e' S S'
-      (BSTEP : ESBasicStep.t e e' S S')
-      (LSTEP: t_load e e' S S') 
-      (wfE: ES.Wf S) :
-  E S' ∩₁ W S' ≡₁ E S ∩₁ W S.
-Proof. cdes LSTEP; cdes AJF. step_type_solver. Qed.  
-
-Lemma load_step_F e e' S S'
-      (BSTEP : ESBasicStep.t e e' S S')
-      (LSTEP: t_load e e' S S') 
-      (wfE: ES.Wf S) :
-  E S' ∩₁ F S' ≡₁ E S ∩₁ F S.
-Proof. cdes LSTEP; cdes AJF. step_type_solver. Qed.  
-
-Lemma load_step_acq e e' S S'
-      (BSTEP : ESBasicStep.t e e' S S')
-      (LSTEP: t_load e e' S S') 
-      (wfE: ES.Wf S) :
-  E S' ∩₁ FR S' ∩₁ Acq S' ≡₁ E S ∩₁ FR S ∩₁ Acq S ∪₁ eq e ∩₁ Acq S'.
-Proof. cdes LSTEP; cdes AJF. step_type_solver. Qed.  
-
-Lemma load_step_Rel e e' S S'
-      (BSTEP : ESBasicStep.t e e' S S')
-      (LSTEP: t_load e e' S S') 
-      (wfE: ES.Wf S) :
-  E S' ∩₁ FW S' ∩₁ Rel S' ≡₁ E S ∩₁ FW S ∩₁ Rel S.
-Proof. cdes LSTEP; cdes AJF. step_type_solver. Qed.  
-
-(******************************************************************************)
-(** ** Store step properties *)
-(******************************************************************************)
-
-Lemma store_step_E e e' S S'
-      (BSTEP : ESBasicStep.t e e' S S')
-      (SSTEP: t_store e e' S S') :
-  E S' ≡₁ E S ∪₁ eq e.
-Proof. cdes SSTEP. subst. by apply ESBasicStep.basic_step_nupd_acts_set. Qed.
-
-Lemma store_step_R e e' S S'
-      (BSTEP : ESBasicStep.t e e' S S')
-      (SSTEP: t_store e e' S S') 
-      (wfE: ES.Wf S) :
-  E S' ∩₁ R S' ≡₁ E S ∩₁ R S.
-Proof. cdes SSTEP; cdes ACO. step_type_solver. Qed.  
-
-Lemma store_step_W e e' S S'
-      (BSTEP : ESBasicStep.t e e' S S')
-      (SSTEP: t_store e e' S S') 
-      (wfE: ES.Wf S) :
-  E S' ∩₁ W S' ≡₁ E S ∩₁ W S ∪₁ eq e.
-Proof. cdes SSTEP; cdes ACO. step_type_solver. Qed.  
-
-Lemma store_step_F e e' S S'
-      (BSTEP : ESBasicStep.t e e' S S')
-      (SSTEP: t_store e e' S S') 
-      (wfE: ES.Wf S) :
-  E S' ∩₁ F S' ≡₁ E S ∩₁ F S.
-Proof. cdes SSTEP; cdes ACO. step_type_solver. Qed.  
-
-Lemma store_step_acq e e' S S'
-      (BSTEP : ESBasicStep.t e e' S S')
-      (SSTEP: t_store e e' S S') 
-      (wfE: ES.Wf S) :
-  E S' ∩₁ FR S' ∩₁ Acq S' ≡₁ E S ∩₁ FR S ∩₁ Acq S.
-Proof. cdes SSTEP; cdes ACO. step_type_solver. Qed.  
-
-Lemma store_step_Rel e e' S S'
-      (BSTEP : ESBasicStep.t e e' S S')
-      (SSTEP: t_store e e' S S') 
-      (wfE: ES.Wf S) :
-  E S' ∩₁ FW S' ∩₁ Rel S' ≡₁ E S ∩₁ FW S ∩₁ Rel S ∪₁ eq e ∩₁ Rel S'.
-Proof. cdes SSTEP; cdes ACO. step_type_solver. Qed.  
-
-(******************************************************************************)
-(** ** Update step properties *)
-(******************************************************************************)
-
-Lemma update_step_E e e' S S'
-      (BSTEP : ESBasicStep.t e (Some e') S S')
-      (USTEP: t_update e (Some e') S S') :
-  E S' ≡₁ E S ∪₁ eq e ∪₁ eq e'.
-Proof. cdes USTEP. erewrite ESBasicStep.basic_step_acts_set; eauto. basic_solver. Qed.
-
-Lemma update_step_R e e' S S'
-      (BSTEP : ESBasicStep.t e (Some e') S S')
-      (USTEP: t_update e (Some e') S S') 
-      (wfE: ES.Wf S) :
-  E S' ∩₁ R S' ≡₁ E S ∩₁ R S ∪₁ eq e.
-Proof. cdes USTEP; cdes AJF; cdes ACO. step_type_solver. Qed.  
-
-Lemma update_step_W e e' S S'
-      (BSTEP : ESBasicStep.t e (Some e') S S')
-      (USTEP: t_update e (Some e') S S') 
-      (wfE: ES.Wf S) :
-  E S' ∩₁ W S' ≡₁ E S ∩₁ W S ∪₁ eq e'.
-Proof. cdes USTEP; cdes AJF; cdes ACO. step_type_solver. Qed.  
-
-Lemma update_step_F e e' S S'
-      (BSTEP : ESBasicStep.t e (Some e') S S')
-      (USTEP: t_update e (Some e') S S') 
-      (wfE: ES.Wf S) :
-  E S' ∩₁ F S' ≡₁ E S ∩₁ F S.
-Proof. cdes USTEP; cdes AJF; cdes ACO. step_type_solver. Qed.  
-
-Lemma update_step_acq e e' S S'
-      (BSTEP : ESBasicStep.t e (Some e') S S')
-      (USTEP: t_update e (Some e') S S') 
-      (wfE: ES.Wf S) :
-  E S' ∩₁ FR S' ∩₁ Acq S' ≡₁ E S ∩₁ FR S ∩₁ Acq S ∪₁ eq e ∩₁ Acq S'.
-Proof. cdes USTEP; cdes AJF; cdes ACO. step_type_solver. Qed.  
-
-Lemma update_step_Rel e e' S S'
-      (BSTEP : ESBasicStep.t e (Some e') S S')
-      (USTEP: t_update e (Some e') S S') 
-      (wfE: ES.Wf S) :
-  E S' ∩₁ FW S' ∩₁ Rel S' ≡₁ E S ∩₁ FW S ∩₁ Rel S ∪₁ (eq e' ∩₁ Rel S').
-Proof. cdes USTEP; cdes AJF; cdes ACO. step_type_solver. Qed.  
-
-End ESstep.
