Coq/src/AddCO.v
@@ -1,0 +1,435 @@
+From hahn Require Import Hahn.
+From imm Require Import Events AuxRel. 
+Require Import AuxRel.
+Require Import AuxDef.
+Require Import EventStructure.
+Require Import Consistency.
+Require Import BasicStep.
+Require Import AddEW.
+
+Set Implicit Arguments.
+
+Notation "'E' S" := S.(ES.acts_set) (at level 10).
+Notation "'Einit' S"  := S.(ES.acts_init_set) (at level 10).
+Notation "'Eninit' S" := S.(ES.acts_ninit_set) (at level 10).
+
+Notation "'tid' S" := S.(ES.tid) (at level 10).
+Notation "'lab' S" := S.(ES.lab) (at level 10).
+Notation "'mod' S" := (Events.mod S.(ES.lab)) (at level 10).
+Notation "'loc' S" := (Events.loc S.(ES.lab)) (at level 10).
+Notation "'val' S" := (Events.val S.(ES.lab)) (at level 10).
+
+Notation "'sb' S" := S.(ES.sb) (at level 10).
+Notation "'rmw' S" := S.(ES.rmw) (at level 10).
+Notation "'ew' S" := S.(ES.ew) (at level 10).
+Notation "'jf' S" := S.(ES.jf) (at level 10).
+Notation "'rf' S" := S.(ES.rf) (at level 10).
+Notation "'co' S" := S.(ES.co) (at level 10).
+Notation "'cf' S" := S.(ES.cf) (at level 10).
+
+Notation "'jfe' S" := S.(ES.jfe) (at level 10).
+Notation "'rfe' S" := S.(ES.rfe) (at level 10).
+Notation "'coe' S" := S.(ES.coe) (at level 10).
+Notation "'jfi' S" := S.(ES.jfi) (at level 10).
+Notation "'rfi' S" := S.(ES.rfi) (at level 10).
+Notation "'coi' S" := S.(ES.coi) (at level 10).
+
+Notation "'R' S" := (fun a => is_true (is_r S.(ES.lab) a)) (at level 10).
+Notation "'W' S" := (fun a => is_true (is_w S.(ES.lab) a)) (at level 10).
+Notation "'F' S" := (fun a => is_true (is_f S.(ES.lab) a)) (at level 10).
+
+Notation "'RW' S" := (R S ∪₁ W S) (at level 10).
+Notation "'FR' S" := (F S ∪₁ R S) (at level 10).
+Notation "'FW' S" := (F S ∪₁ W S) (at level 10).
+
+Notation "'Pln' S" := (fun a => is_true (is_only_pln S.(ES.lab) a)) (at level 10).
+Notation "'Rlx' S" := (fun a => is_true (is_rlx S.(ES.lab) a)) (at level 10).
+Notation "'Rel' S" := (fun a => is_true (is_rel S.(ES.lab) a)) (at level 10).
+Notation "'Acq' S" := (fun a => is_true (is_acq S.(ES.lab) a)) (at level 10).
+Notation "'Acqrel' S" := (fun a => is_true (is_acqrel S.(ES.lab) a)) (at level 10).
+Notation "'Sc' S" := (fun a => is_true (is_sc S.(ES.lab) a)) (at level 10).
+
+(* Notation "'same_mod' S" := (same_mod S.(ES.lab)) (at level 10). *)
+(* Notation "'same_loc' S" := (same_loc S.(ES.lab)) (at level 10). *)
+(* Notation "'same_val' S" := (same_val S.(ES.lab)) (at level 10). *)
+
+Notation "'K' S" := (S.(ES.cont_set)) (at level 10).
+
+Notation "'Tid' S" := (fun t e => S.(ES.tid) e = t) (at level 9).
+Notation "'Mod_' S" := (fun m x => mod S x = m) (at level 9).
+Notation "'Loc_' S" := (fun l x => loc S x = l) (at level 9).
+Notation "'Val_' S" := (fun v e => val S e = v) (at level 9).
+
+Definition ws_compl ews ws S := 
+  codom_rel (⦗ews ∪₁ ws⦘ ⨾ co S) \₁ (ews ∪₁ ws).
+
+Definition co_delta ews ws w' S : relation eventid := 
+  ws × eq w' ∪ eq w' × ws_compl ews ws S.
+
+Hint Unfold ws_compl co_delta : ESStepDb.
+
+Definition add_co ews ws w' S S' : Prop := 
+  ⟪ wE' : E S' w' ⟫ /\
+  ⟪ wW' : W S' w' ⟫ /\
+  ⟪ wsE : ws ⊆₁ E S ⟫ /\
+  ⟪ wsW : ws ⊆₁ W S ⟫ /\
+  ⟪ wsLOC : ws ⊆₁ same_loc S' w' ⟫ /\
+  ⟪ ws_ews : ws ∩₁ ews ⊆₁ ∅ ⟫ /\
+  ⟪ wsEinit : (Einit S ∩₁ Loc_ S (loc S' w')) ⊆₁ ws ⟫ /\
+  ⟪ wsCOEWprcl : dom_rel ((co S)^? ⨾ (ew S)^? ⨾ ⦗ws⦘) ⊆₁ ws ⟫ /\
+  ⟪ ewsCOprcl : dom_rel (co S ⨾ ⦗ews⦘) ⊆₁ ws ⟫ /\
+  ⟪ ewsCOprcl : dom_rel (co S ⨾ ⦗ews⦘) ⊆₁ ws ⟫ /\
+  (* ⟪ wsNCF : ws ⊆₁ dom_rel ((co S)^? ⨾ (ew S)^? ⨾ ⦗set_compl (cf S' w')⦘) ⟫ /\ *)
+  ⟪ CO' : co S' ≡ co S ∪ co_delta ews ws w' S ⟫.
+
+(******************************************************************************)
+(** ** ews, ws, ws_compl lemmas *)
+(******************************************************************************)
+
+Lemma add_co_ws_co_prcl ews ws w' S S'
+      (wf : ES.Wf S) 
+      (ACO : add_co ews ws w' S S') : 
+  dom_rel (co S ⨾ ⦗ws⦘) ⊆₁ ws.
+Proof. cdes ACO. generalize wsCOEWprcl. basic_solver 10. Qed.
+
+Lemma add_co_ws_ew_prcl ews ws w' S S'
+      (wf : ES.Wf S) 
+      (ACO : add_co ews ws w' S S') : 
+  dom_rel (ew S ⨾ ⦗ws⦘) ⊆₁ ws.
+Proof. cdes ACO. generalize wsCOEWprcl. basic_solver 10. Qed.
+
+Lemma add_co_ws_ew_fwcl ews ws w' S S'
+      (wf : ES.Wf S) 
+      (ACO : add_co ews ws w' S S') : 
+  codom_rel (⦗ws⦘ ⨾ ew S) ⊆₁ ws.
+Proof. 
+  cdes ACO. 
+  intros x [y [z [[EQz WS] EW]]]. subst z.
+  apply ES.ew_sym in EW; auto.
+  eapply add_co_ws_ew_prcl; eauto.
+  basic_solver 10.
+Qed.
+
+Lemma add_co_ws_co_ew_prcl ews ws w' S S'
+      (wf : ES.Wf S) 
+      (ACO : add_co ews ws w' S S') : 
+  dom_rel (co S ⨾ ew S ⨾ ⦗ws⦘) ⊆₁ ws.
+Proof. cdes ACO. generalize wsCOEWprcl. basic_solver 10. Qed.
+
+Lemma add_co_ws_complE ews ws S 
+      (wf : ES.Wf S) : 
+  ws_compl ews ws S ⊆₁ E S.
+Proof. 
+  unfold ws_compl.
+  rewrite ES.coE; auto.
+  basic_solver.
+Qed.
+
+Lemma add_co_ws_complW ews ws S 
+      (wf : ES.Wf S) : 
+  ws_compl ews ws S ⊆₁ W S.
+Proof. 
+  unfold ws_compl.
+  rewrite ES.coD; auto.
+  basic_solver.
+Qed.
+
+Lemma add_co_ws_compl_loc ews ws w' e e' S S'
+      (wf : ES.Wf S) 
+      (BSTEP : basic_step e e' S S') 
+      (AEW : add_ew ews w' S S')
+      (ACO : add_co ews ws w' S S') : 
+  ws_compl ews ws S ⊆₁ same_loc S' w'.
+Proof. 
+  cdes AEW; cdes ACO.
+  unfold ws_compl.
+  rewrite ES.coE; auto.
+  rewrite ewsLOC at 1.
+  rewrite wsLOC at 1.
+  rewrite ES.col; auto.
+  rewrite set_unionK.
+  intros x [[y HH] _].
+  unfolder in HH. desc.
+  etransitivity; eauto.
+  arewrite (loc S' y = loc S y).
+  { erewrite basic_step_loc_eq_dom; eauto. }
+  arewrite (loc S' x = loc S x).
+  { erewrite basic_step_loc_eq_dom; eauto. }
+  done. 
+Qed.
+
+Lemma add_co_wsEWLoc ews ws w' e e' S S'
+      (wf : ES.Wf S) 
+      (BSTEP : basic_step e e' S S') 
+      (ACO : add_co ews ws w' S S') : 
+  ws ⊆₁ (E S) ∩₁ (W S) ∩₁ (Loc_ S (loc S' w')).
+Proof. 
+  cdes ACO.
+  intros x xWS.
+  unfolder; splits; auto.
+  etransitivity.
+  { symmetry. eapply basic_step_loc_eq_dom; eauto. }
+  symmetry. by apply wsLOC in xWS.
+Qed.
+
+Lemma add_co_ws_complEWLoc ews ws w' e e' S S'
+      (wf : ES.Wf S) 
+      (BSTEP : basic_step e e' S S') 
+      (AEW : add_ew ews w' S S')
+      (ACO : add_co ews ws w' S S') : 
+  ws_compl ews ws S ⊆₁ (E S) ∩₁ (W S) ∩₁ (Loc_ S (loc S' w')).
+Proof. 
+  cdes ACO.
+  intros x xWS.
+  unfolder; splits; auto.
+  { eapply add_co_ws_complE; eauto. }
+  { eapply add_co_ws_complW; eauto. }
+  etransitivity.
+  { symmetry. eapply basic_step_loc_eq_dom; eauto. 
+    eapply add_co_ws_complE; eauto. }
+  symmetry. eapply add_co_ws_compl_loc in xWS; eauto. 
+Qed.
+
+Lemma add_co_ws_compl_co_fwcl ews ws w' S S'
+      (wf : ES.Wf S) 
+      (ACO : add_co ews ws w' S S') : 
+  codom_rel (⦗ws_compl ews ws S⦘ ⨾ co S) ⊆₁ ws_compl ews ws S.
+Proof. 
+  cdes ACO. 
+  unfold ws_compl. 
+  intros y [x [z [[EQz HH] CO]]]. subst z.
+  destruct HH as [[z [z' [[EQz' EWWS] COzx]]] nEWWS]. subst z'.
+  red. splits.
+  { do 2 eexists. splits. 
+    { red. eauto using EWWS. }
+    eapply ES.co_trans; eauto. }
+  intros EWWSy. apply nEWWS.
+  generalize wsCOEWprcl ewsCOprcl EWWSy CO.
+  basic_solver 10.
+Qed.
+
+Lemma add_co_ws_compl_ew_fwcl ews ws w' S S'
+      (wf : ES.Wf S) 
+      (AEW : add_ew ews w' S S')
+      (ACO : add_co ews ws w' S S') : 
+  codom_rel (⦗ws_compl ews ws S⦘ ⨾ ew S) ⊆₁ ws_compl ews ws S.
+Proof. 
+  cdes AEW; cdes ACO. 
+  unfold ws_compl. 
+  intros y [x [z [[EQz HH] EW]]]. subst z.
+  destruct HH as [[z [z' [[EQz' EWWS] COzx]]] nEWWS]. subst z'.
+  red. splits.
+  { do 2 eexists. splits. 
+    { red. eauto using EWWS. }
+    eapply ES.co_ew_in_co; eauto. 
+    basic_solver. }
+  intros EWWSy. apply nEWWS.
+  generalize wsCOEWprcl ewsCOprcl EWWSy ewsEWprcl EW.
+  basic_solver 10.
+Qed.
+
+Lemma add_co_ws_inter_ws_compl_false ews ws w' S S'
+      (wf : ES.Wf S) 
+      (ACO : add_co ews ws w' S S') : 
+  ws ∩₁ ws_compl ews ws S ⊆₁ ∅.
+Proof. unfold ws_compl. basic_solver. Qed.
+
+Lemma add_co_ews_inter_ws_compl_false ews ws w' S S'
+      (wf : ES.Wf S) 
+      (ACO : add_co ews ws w' S S') : 
+  ews ∩₁ ws_compl ews ws S ⊆₁ ∅.
+Proof. unfold ws_compl. basic_solver. Qed.
+
+Lemma add_co_ws_cross_ws_compl_in_co ews ws w' e e' S S'
+      (wf : ES.Wf S) 
+      (BSTEP : basic_step e e' S S') 
+      (AEW : add_ew ews w' S S')
+      (ACO : add_co ews ws w' S S') 
+      (wEE' : (eq e ∪₁ eq_opt e') w') : 
+  ws × ws_compl ews ws S ⊆ co S.
+Proof. 
+  cdes AEW; cdes ACO.
+  intros x y [xWS yWS].
+  destruct 
+    (excluded_middle_informative (ew S x y))
+    as [EW | nEW].
+  { exfalso.
+    destruct yWS as [HH nEWWS].
+    eapply nEWWS.
+    right. eapply add_co_ws_ew_fwcl; eauto. 
+    basic_solver 10. }
+  edestruct ES.co_total; eauto.
+  { eapply add_co_wsEWLoc; eauto. }
+  { eapply add_co_ws_complEWLoc; eauto. }
+  exfalso. 
+  destruct yWS as [HH nEWWS].
+  apply nEWWS.
+  right. eapply add_co_ws_co_prcl; eauto.
+  basic_solver 10. 
+Qed.
+
+Lemma add_co_ws_cross_ews_in_ew_compl ews ws w' e e' S S'
+      (wf : ES.Wf S)
+      (BSTEP : basic_step e e' S S')
+      (AEW : add_ew ews w' S S')
+      (ACO : add_co ews ws w' S S')
+      (wEE' : (eq e ∪₁ eq_opt e') w') :
+  ws × ews ⊆ compl_rel (ew S).
+Proof.
+  cdes AEW; cdes ACO.
+  intros x y [xWS yEWS].
+  assert (~ ews x) as xnEWS.
+  { red. ins. eapply ws_ews; eauto. basic_solver. }
+  intros EW. eapply ws_ews; eauto.
+  split; [|eauto].
+  eapply add_co_ws_ew_fwcl; eauto.
+  basic_solver 10.
+Qed.
+
+Lemma add_co_ews_cross_ws_compl_in_ew_compl ews ws w' e e' S S'
+      (wf : ES.Wf S) 
+      (BSTEP : basic_step e e' S S') 
+      (AEW : add_ew ews w' S S')
+      (ACO : add_co ews ws w' S S') 
+      (wEE' : (eq e ∪₁ eq_opt e') w') : 
+  ews × ws_compl ews ws S ⊆ compl_rel (ew S).
+Proof. 
+  cdes AEW; cdes ACO.
+  intros x y [xEWS yWSC].
+  assert (~ ews y) as ynEWS.
+  { red. ins. eapply add_co_ews_inter_ws_compl_false; eauto. basic_solver. }
+  intros EW. eapply add_co_ews_inter_ws_compl_false; eauto.
+  split; [|eauto].
+  eapply add_ew_ews_ew_fwcl; eauto.
+  basic_solver 10.
+Qed.
+
+Lemma add_co_ws_cross_ews_in_co ews ws w' e e' S S'
+      (wf : ES.Wf S) 
+      (BSTEP : basic_step e e' S S') 
+      (AEW : add_ew ews w' S S')
+      (ACO : add_co ews ws w' S S') 
+      (wEE' : (eq e ∪₁ eq_opt e') w') : 
+  ws × ews ⊆ co S.
+Proof. 
+  cdes AEW; cdes ACO.
+  intros x y [xWS yEWS].
+  assert (~ ew S x y) as nEW.
+  { eapply add_co_ws_cross_ews_in_ew_compl; eauto. basic_solver. }
+  edestruct ES.co_total as [COxy | COyx]; eauto.
+  { eapply add_co_wsEWLoc; eauto. }
+  { eapply add_ew_ewsEWLoc; eauto. }
+  exfalso. eapply ws_ews.
+  split; [|eauto].
+  eapply add_co_ws_co_prcl; eauto.
+  basic_solver 10.
+Qed.
+
+Lemma add_co_ews_cross_ws_compl_in_co ews ws w' e e' S S'
+      (wf : ES.Wf S) 
+      (BSTEP : basic_step e e' S S') 
+      (AEW : add_ew ews w' S S')
+      (ACO : add_co ews ws w' S S') 
+      (wEE' : (eq e ∪₁ eq_opt e') w') : 
+  ews × ws_compl ews ws S ⊆ co S.
+Proof. 
+  cdes AEW; cdes ACO.
+  intros x y [xEWS yWSC].
+  assert (~ ew S x y) as nEW.
+  { eapply add_co_ews_cross_ws_compl_in_ew_compl; eauto. basic_solver. }
+  set (yWSC' := yWSC).
+  destruct yWSC' as [[z [z' [[EQz' HA] CO]]] HB]. subst z'.
+  destruct HA as [zEWS | zWS].
+  { apply ES.ew_co_in_co; auto.
+    eexists; splits; eauto. 
+    apply ewsEW. basic_solver. }
+  edestruct ES.co_total as [COxy | COyx]; eauto.
+  { eapply add_ew_ewsEWLoc; eauto. }
+  { eapply add_co_ws_complEWLoc; eauto. }
+  exfalso. eapply HB.
+  right. apply ewsCOprcl. basic_solver 10.
+Qed.
+
+Lemma add_co_ews_co_codom ews ws w' S S'
+      (wf : ES.Wf S) 
+      (AEW : add_ew ews w' S S')
+      (ACO : add_co ews ws w' S S') : 
+  codom_rel (⦗ews⦘ ⨾ co S) ⊆₁ ws_compl ews ws S. 
+Proof. 
+  cdes AEW; cdes ACO.
+  unfold ws_compl.
+  intros x [y [z [[EQz EWS] CO]]]. subst z.
+  unfolder; splits; eauto 10.
+  intros [EW | WS].
+  { eapply ES.ew_co; eauto.
+    split; eauto.
+    eapply ewsEW. 
+    basic_solver. }
+  eapply ws_ews. split; [|eauto].
+  eapply add_co_ws_co_prcl; eauto. basic_solver 10. 
+Qed.
+
+Lemma add_co_ews_co_ws_empty ews ws w' S S'
+      (wf : ES.Wf S) 
+      (AEW : add_ew ews w' S S')
+      (ACO : add_co ews ws w' S S') : 
+  ⦗ews⦘ ⨾ co S ⨾ ⦗ws⦘ ⊆ ∅₂.
+Proof. 
+  cdes AEW; cdes ACO.
+  rewrite <- seqA.
+  intros x y [z [HA [EQz WSy]]]. subst z.
+  eapply add_co_ws_inter_ws_compl_false; eauto.
+  split; eauto.
+  eapply add_co_ews_co_codom; eauto.
+  basic_solver.
+Qed.
+
+(******************************************************************************)
+(** ** co_delta lemmas *)
+(******************************************************************************)
+
+Lemma add_co_co_delta_dom ews ws w' e e' S S'
+      (BSTEP : basic_step e e' S S') 
+      (ACO : add_co ews ws w' S S') 
+      (wf : ES.Wf S) 
+      (wEE' : (eq e ∪₁ eq_opt e') w') : 
+  dom_rel (co_delta ews ws w' S) ⊆₁ ws ∪₁ eq w'.
+Proof. unfold co_delta. basic_solver. Qed.
+
+Lemma add_co_co_delta_codom ews ws w' e e' S S'
+      (BSTEP : basic_step e e' S S') 
+      (ACO : add_co ews ws w' S S') 
+      (wf : ES.Wf S) 
+      (wEE' : (eq e ∪₁ eq_opt e') w') : 
+  codom_rel (co_delta ews ws w' S) ⊆₁ ws_compl ews ws S ∪₁ eq w'.
+Proof. unfold co_delta. basic_solver. Qed.
+
+Lemma add_co_co_deltaEl ews ws w' e e' S S'
+      (BSTEP : basic_step e e' S S') 
+      (ACO : add_co ews ws w' S S') 
+      (wf : ES.Wf S) 
+      (wEE' : (eq e ∪₁ eq_opt e') w') : 
+  co_delta ews ws w' S ⨾ ⦗E S⦘ ≡ eq w' × ws_compl ews ws S.
+Proof. 
+  cdes ACO; cdes BSTEP; cdes BSTEP_.
+  unfold co_delta. relsf.
+  arewrite_false (ws × eq w' ⨾ ⦗E S⦘).
+  { unfolder in wEE'; desf; step_solver. }
+  relsf. split; [basic_solver|].
+  unfolder. ins. desf. splits; auto.
+  eapply add_co_ws_complE; eauto.
+Qed.  
+
+Lemma add_co_co_deltaEr ews ws w' e e' S S'
+      (BSTEP : basic_step e e' S S') 
+      (ACO : add_co ews ws w' S S') 
+      (wf : ES.Wf S) 
+      (wEE' : (eq e ∪₁ eq_opt e') w') : 
+  ⦗E S⦘ ⨾ co_delta ews ws w' S ≡ ws × eq w'.
+Proof. 
+  cdes ACO; cdes BSTEP; cdes BSTEP_.
+  unfold co_delta. relsf.
+  arewrite_false (⦗E S⦘ ⨾ eq w' × ws_compl ews ws S). 
+  { unfolder in wEE'; desf; step_solver. }
+  basic_solver 10.
+Qed.  
