Coq/src/AddEW.v
@@ -1,0 +1,167 @@
+From hahn Require Import Hahn.
+From imm Require Import Events AuxRel. 
+Require Import AuxRel.
+Require Import AuxDef.
+Require Import EventStructure.
+Require Import Consistency.
+Require Import BasicStep.
+
+Set Implicit Arguments.
+
+Notation "'E' S" := S.(ES.acts_set) (at level 10).
+Notation "'Einit' S"  := S.(ES.acts_init_set) (at level 10).
+Notation "'Eninit' S" := S.(ES.acts_ninit_set) (at level 10).
+
+Notation "'tid' S" := S.(ES.tid) (at level 10).
+Notation "'lab' S" := S.(ES.lab) (at level 10).
+Notation "'mod' S" := (Events.mod S.(ES.lab)) (at level 10).
+Notation "'loc' S" := (Events.loc S.(ES.lab)) (at level 10).
+Notation "'val' S" := (Events.val S.(ES.lab)) (at level 10).
+
+Notation "'sb' S" := S.(ES.sb) (at level 10).
+Notation "'rmw' S" := S.(ES.rmw) (at level 10).
+Notation "'ew' S" := S.(ES.ew) (at level 10).
+Notation "'jf' S" := S.(ES.jf) (at level 10).
+Notation "'rf' S" := S.(ES.rf) (at level 10).
+Notation "'co' S" := S.(ES.co) (at level 10).
+Notation "'cf' S" := S.(ES.cf) (at level 10).
+
+Notation "'jfe' S" := S.(ES.jfe) (at level 10).
+Notation "'rfe' S" := S.(ES.rfe) (at level 10).
+Notation "'coe' S" := S.(ES.coe) (at level 10).
+Notation "'jfi' S" := S.(ES.jfi) (at level 10).
+Notation "'rfi' S" := S.(ES.rfi) (at level 10).
+Notation "'coi' S" := S.(ES.coi) (at level 10).
+
+Notation "'R' S" := (fun a => is_true (is_r S.(ES.lab) a)) (at level 10).
+Notation "'W' S" := (fun a => is_true (is_w S.(ES.lab) a)) (at level 10).
+Notation "'F' S" := (fun a => is_true (is_f S.(ES.lab) a)) (at level 10).
+
+Notation "'RW' S" := (R S ∪₁ W S) (at level 10).
+Notation "'FR' S" := (F S ∪₁ R S) (at level 10).
+Notation "'FW' S" := (F S ∪₁ W S) (at level 10).
+
+Notation "'Pln' S" := (fun a => is_true (is_only_pln S.(ES.lab) a)) (at level 10).
+Notation "'Rlx' S" := (fun a => is_true (is_rlx S.(ES.lab) a)) (at level 10).
+Notation "'Rel' S" := (fun a => is_true (is_rel S.(ES.lab) a)) (at level 10).
+Notation "'Acq' S" := (fun a => is_true (is_acq S.(ES.lab) a)) (at level 10).
+Notation "'Acqrel' S" := (fun a => is_true (is_acqrel S.(ES.lab) a)) (at level 10).
+Notation "'Sc' S" := (fun a => is_true (is_sc S.(ES.lab) a)) (at level 10).
+
+(* Notation "'same_mod' S" := (same_mod S.(ES.lab)) (at level 10). *)
+(* Notation "'same_loc' S" := (same_loc S.(ES.lab)) (at level 10). *)
+(* Notation "'same_val' S" := (same_val S.(ES.lab)) (at level 10). *)
+
+Notation "'K' S" := (S.(ES.cont_set)) (at level 10).
+
+Notation "'Tid' S" := (fun t e => S.(ES.tid) e = t) (at level 9).
+Notation "'Mod_' S" := (fun m x => mod S x = m) (at level 9).
+Notation "'Loc_' S" := (fun l x => loc S x = l) (at level 9).
+Notation "'Val_' S" := (fun v e => val S e = v) (at level 9).
+
+Definition ew_delta ws w : relation eventid := 
+  eq w × eq w ∪ (ws × eq w)^⋈.
+
+Hint Unfold ew_delta : ESStepDb.
+
+Definition add_ew ews w' S S' : Prop :=   
+  ⟪ wE' : E S' w' ⟫ /\
+  ⟪ wW' : W S' w' ⟫ /\
+  ⟪ ewsE : ews ⊆₁ E S ⟫ /\
+  ⟪ ewsW : ews ⊆₁ W S ⟫ /\
+  ⟪ ewsRLX : ews ⊆₁ Rlx S ⟫ /\
+  ⟪ ewsMOD : ews ⊆₁ same_mod S' w' ⟫ /\
+  ⟪ ewsLOC : ews ⊆₁ same_loc S' w' ⟫ /\
+  ⟪ ewsVAL : ews ⊆₁ same_val S' w' ⟫ /\
+  ⟪ ewsCF : ews ⊆₁ cf S' w' ⟫ /\
+  ⟪ ewsEW : ews × ews ⊆ ew S ⟫ /\
+  ⟪ ewsEWprcl : dom_rel (ew S ⨾ ⦗ews⦘) ⊆₁ ews ⟫ /\
+  ⟪ EW' : ew S' ≡ ew S ∪ ew_delta ews w' ⟫. 
+
+(******************************************************************************)
+(** ** ews lemmas *)
+(******************************************************************************)
+
+Lemma add_ew_ewsEWLoc ews w' e e' S S'
+      (wf : ES.Wf S) 
+      (BSTEP : basic_step e e' S S') 
+      (AEW : add_ew ews w' S S') : 
+  ews ⊆₁ (E S) ∩₁ (W S) ∩₁ (Loc_ S (loc S' w')).
+Proof. 
+  cdes AEW.
+  intros x xEWS.
+  unfolder; splits; auto.
+  etransitivity.
+  { symmetry. eapply basic_step_loc_eq_dom; eauto. }
+  symmetry. by apply ewsLOC in xEWS.
+Qed.
+
+Lemma add_ew_ews_ew_fwcl ews w' S S'
+      (wf : ES.Wf S) 
+      (AEW : add_ew ews w' S S') : 
+  codom_rel (⦗ews⦘ ⨾ ew S) ⊆₁ ews.
+Proof.
+  cdes AEW. 
+  intros x [y [z [[EQz EWS] EW]]]. subst z.
+  apply ES.ew_sym in EW; auto.
+  apply ewsEWprcl.
+  basic_solver 10.
+Qed.
+
+(******************************************************************************)
+(** ** ew_delta lemmas *)
+(******************************************************************************)
+
+Lemma add_ew_ew_delta_dom ews w' e e' S S'
+      (BSTEP : basic_step e e' S S') 
+      (AEW : add_ew ews w' S S') 
+      (wf : ES.Wf S) 
+      (wEE' : (eq e ∪₁ eq_opt e') w') : 
+  dom_rel (ew_delta ews w') ⊆₁ ews ∪₁ eq w'.
+Proof. unfold ew_delta. basic_solver. Qed.
+
+Lemma add_ew_ew_delta_codom ews w' e e' S S'
+      (BSTEP : basic_step e e' S S') 
+      (AEW : add_ew ews w' S S') 
+      (wf : ES.Wf S) 
+      (wEE' : (eq e ∪₁ eq_opt e') w') : 
+  codom_rel (ew_delta ews w') ⊆₁ ews ∪₁ eq w'.
+Proof. unfold ew_delta. basic_solver. Qed.
+
+Lemma add_ew_ew_deltaEl ews w' e e' S S'
+      (BSTEP : basic_step e e' S S') 
+      (AEW : add_ew ews w' S S') 
+      (wf : ES.Wf S) 
+      (wEE' : (eq e ∪₁ eq_opt e') w') : 
+  ew_delta ews w' ⨾ ⦗E S⦘ ≡ eq w' × ews. 
+Proof. 
+  cdes AEW; cdes BSTEP; cdes BSTEP_.
+  unfold ew_delta. 
+  rewrite csE, transp_cross.
+  relsf.
+  arewrite_false (eq w' × eq w' ⨾ ⦗E S⦘).
+  { unfolder in wEE'; desf; step_solver. }
+  arewrite_false (ews × eq w' ⨾ ⦗E S⦘).
+  { unfolder in wEE'; desf; step_solver. }
+  relsf. 
+  generalize ewsE. basic_solver.
+Qed.
+
+Lemma add_ew_ew_deltaEr ews w' e e' S S'
+      (BSTEP : basic_step e e' S S') 
+      (AEW : add_ew ews w' S S') 
+      (wf : ES.Wf S) 
+      (wEE' : (eq e ∪₁ eq_opt e') w') : 
+  ⦗E S⦘ ⨾ ew_delta ews w' ≡ ews × eq w'. 
+Proof. 
+  cdes AEW; cdes BSTEP; cdes BSTEP_.
+  unfold ew_delta. 
+  rewrite csE, transp_cross.
+  relsf.
+  arewrite_false (⦗E S⦘ ⨾ eq w' × eq w').
+  { unfolder in wEE'; desf; step_solver. }
+  arewrite_false (⦗E S⦘ ⨾ eq w' × ews).
+  { unfolder in wEE'; desf; step_solver. }
+  relsf. 
+  generalize ewsE. basic_solver.
+Qed.
