Coq/src/AddJF.v
@@ -1,0 +1,934 @@
+From hahn Require Import Hahn.
+From imm Require Import Events AuxRel. 
+Require Import AuxRel.
+Require Import AuxDef.
+Require Import EventStructure.
+Require Import Consistency.
+Require Import BasicStep.
+
+Set Implicit Arguments.
+
+Notation "'E' S" := S.(ES.acts_set) (at level 10).
+Notation "'Einit' S"  := S.(ES.acts_init_set) (at level 10).
+Notation "'Eninit' S" := S.(ES.acts_ninit_set) (at level 10).
+
+Notation "'tid' S" := S.(ES.tid) (at level 10).
+Notation "'lab' S" := S.(ES.lab) (at level 10).
+Notation "'mod' S" := (Events.mod S.(ES.lab)) (at level 10).
+Notation "'loc' S" := (Events.loc S.(ES.lab)) (at level 10).
+Notation "'val' S" := (Events.val S.(ES.lab)) (at level 10).
+
+Notation "'sb' S" := S.(ES.sb) (at level 10).
+Notation "'rmw' S" := S.(ES.rmw) (at level 10).
+Notation "'ew' S" := S.(ES.ew) (at level 10).
+Notation "'jf' S" := S.(ES.jf) (at level 10).
+Notation "'rf' S" := S.(ES.rf) (at level 10).
+Notation "'co' S" := S.(ES.co) (at level 10).
+Notation "'cf' S" := S.(ES.cf) (at level 10).
+
+Notation "'jfe' S" := S.(ES.jfe) (at level 10).
+Notation "'rfe' S" := S.(ES.rfe) (at level 10).
+Notation "'coe' S" := S.(ES.coe) (at level 10).
+Notation "'jfi' S" := S.(ES.jfi) (at level 10).
+Notation "'rfi' S" := S.(ES.rfi) (at level 10).
+Notation "'coi' S" := S.(ES.coi) (at level 10).
+
+Notation "'R' S" := (fun a => is_true (is_r S.(ES.lab) a)) (at level 10).
+Notation "'W' S" := (fun a => is_true (is_w S.(ES.lab) a)) (at level 10).
+Notation "'F' S" := (fun a => is_true (is_f S.(ES.lab) a)) (at level 10).
+
+Notation "'RW' S" := (R S ∪₁ W S) (at level 10).
+Notation "'FR' S" := (F S ∪₁ R S) (at level 10).
+Notation "'FW' S" := (F S ∪₁ W S) (at level 10).
+
+Notation "'Pln' S" := (fun a => is_true (is_only_pln S.(ES.lab) a)) (at level 10).
+Notation "'Rlx' S" := (fun a => is_true (is_rlx S.(ES.lab) a)) (at level 10).
+Notation "'Rel' S" := (fun a => is_true (is_rel S.(ES.lab) a)) (at level 10).
+Notation "'Acq' S" := (fun a => is_true (is_acq S.(ES.lab) a)) (at level 10).
+Notation "'Acqrel' S" := (fun a => is_true (is_acqrel S.(ES.lab) a)) (at level 10).
+Notation "'Sc' S" := (fun a => is_true (is_sc S.(ES.lab) a)) (at level 10).
+
+(* Notation "'same_mod' S" := (same_mod S.(ES.lab)) (at level 10). *)
+(* Notation "'same_loc' S" := (same_loc S.(ES.lab)) (at level 10). *)
+(* Notation "'same_val' S" := (same_val S.(ES.lab)) (at level 10). *)
+
+Notation "'K' S" := (S.(ES.cont_set)) (at level 10).
+
+Notation "'Tid' S" := (fun t e => S.(ES.tid) e = t) (at level 9).
+Notation "'Mod_' S" := (fun m x => mod S x = m) (at level 9).
+Notation "'Loc_' S" := (fun l x => loc S x = l) (at level 9).
+Notation "'Val_' S" := (fun v e => val S e = v) (at level 9).
+
+Definition jf_delta w r : relation eventid := 
+  singl_rel w r.
+
+Hint Unfold jf_delta : ESStepDb.
+
+Definition add_jf w r' S S' : Prop :=  
+  ⟪ rE' : E S' r' ⟫ /\
+  ⟪ rR' : R S' r' ⟫ /\
+  ⟪ wE : E S w ⟫ /\
+  ⟪ wW : W S w ⟫ /\
+  ⟪ LOC : same_loc S' w r' ⟫ /\
+  ⟪ VAL : same_val S' w r' ⟫ /\
+  ⟪ nCF : ~ cf S' w r' ⟫ /\
+  ⟪ JF' : jf S' ≡ jf S ∪ jf_delta w r' ⟫.
+
+(******************************************************************************)
+(** ** Deltas definitions *)
+(******************************************************************************)
+
+Definition jfi_delta S k w r : relation eventid := 
+  ⦗ES.cont_sb_dom S k⦘ ⨾ jf_delta w r.
+
+Definition jfe_delta S k w r : relation eventid := 
+  ⦗set_compl (ES.cont_sb_dom S k)⦘ ⨾ jf_delta w r.
+
+Definition sw_delta S S' k e e' : relation eventid := 
+  release S ⨾ (jf S ⨾ sb_delta S k e e' ⨾ ⦗F S'⦘ ∪ jf S' ⨾ ⦗eq e⦘) ⨾ ⦗Acq S'⦘.
+
+Definition hb_delta S S' k e e' : relation eventid := 
+  (hb S)^? ⨾ (sb_delta S k e e' ∪ sw_delta S S' k e e') ⨾ (eq e × eq_opt e')^? . 
+
+Hint Unfold jfi_delta jfe_delta sw_delta hb_delta : ESStepDb.
+
+(******************************************************************************)
+(** ** Auxiliary lemmas *)
+(******************************************************************************)
+
+Lemma basic_step_w_sb_loc_wE e e' S S'
+      (BSTEP : basic_step e e' S S') 
+      (wfE: ES.Wf S) :
+  ⦗E S' ∩₁ W S'⦘ ⨾ (sb S' ∩ same_loc S')^? ⨾ ⦗W S'⦘ ⨾ ⦗E S⦘ ≡ 
+  ⦗E S  ∩₁ W S ⦘ ⨾ (sb S  ∩ same_loc S )^? ⨾ ⦗W S ⦘.
+Proof. 
+  cdes BSTEP. cdes BSTEP_.
+  arewrite (⦗W S'⦘ ⨾ ⦗E S⦘ ≡ ⦗E S⦘ ⨾ ⦗W S⦘). 
+  { rewrite seq_eqvC.
+    rewrite !seq_eqv.
+    apply eqv_rel_more.
+    eapply basic_step_w_eq_w; eauto. }
+  arewrite ((sb S' ∩ same_loc S')^? ⨾ ⦗E S⦘ ≡ ⦗E S⦘ ⨾ (sb S ∩ same_loc S)^?).
+  { rewrite !crE. relsf.
+    apply union_more; auto.
+    rewrite <- lib.AuxRel.seq_eqv_inter_lr.
+    rewrite basic_step_sbE; eauto.
+    rewrite ES.sbE at 1; auto.
+    rewrite <- restr_relE, <- restr_inter_absorb_r.
+    rewrite basic_step_same_loc_restr; eauto.
+    rewrite restr_inter_absorb_r, restr_relE.
+    rewrite ES.sbE; auto.
+    basic_solver 20. }
+  arewrite (⦗E S' ∩₁ W S'⦘ ⨾ ⦗E S⦘ ≡ ⦗E S ∩₁ W S⦘).
+  { rewrite basic_step_acts_set; eauto.
+    rewrite !set_inter_union_l, !id_union. relsf.
+    arewrite_false (⦗eq e ∩₁ W S'⦘ ⨾ ⦗E S⦘).
+    { step_solver. }
+    arewrite_false (⦗eq_opt e' ∩₁ W S'⦘ ⨾ ⦗E S⦘).
+    { step_solver. }
+    relsf. 
+    rewrite basic_step_w_eq_w; eauto.
+    basic_solver. }
+  done.
+Qed.
+
+Lemma basic_step_rel_f_sbE e e' S S'
+      (BSTEP : basic_step e e' S S') 
+      (wfE: ES.Wf S) :
+  ⦗Rel S'⦘ ⨾ (⦗F S'⦘ ⨾ sb S')^? ⨾ ⦗E S⦘ ≡ 
+  ⦗Rel S ⦘ ⨾ (⦗F S ⦘ ⨾ sb S )^? ⨾ ⦗E S⦘.
+Proof. 
+  arewrite ((⦗F S'⦘ ⨾ sb S')^? ⨾ ⦗E S⦘ ≡ ⦗E S⦘ ⨾ (⦗F S⦘ ⨾ sb S)^?).
+  { rewrite !crE. relsf.
+    apply union_more; auto.
+    rewrite !seqA.
+    rewrite basic_step_sbE; eauto.
+    rewrite ES.sbE; auto.
+    arewrite (⦗F S'⦘ ⨾ ⦗E S⦘ ≡ ⦗E S⦘ ⨾ ⦗F S⦘).
+    { rewrite !seq_eqv.
+      apply eqv_rel_more.
+      rewrite set_interC.
+      eapply basic_step_f_eq_f; eauto. }
+    basic_solver. }
+  arewrite (⦗Rel S'⦘ ⨾ ⦗E S⦘ ≡ ⦗Rel S⦘ ⨾ ⦗E S⦘).
+  { rewrite !seq_eqv.
+    apply eqv_rel_more.
+    rewrite set_interC.
+    autorewrite with same_lab_solveDb; eauto.
+    basic_solver. }
+  rewrite ES.sbE; auto.
+  basic_solver 10.
+Qed.
+
+Lemma basic_step_jf_sb_f_acq e e' S S'
+      (BSTEP : basic_step e e' S S') 
+      (WF: ES.Wf S) :
+  jf S ⨾ (sb S ⨾ ⦗F S'⦘)^? ⨾ ⦗Acq S'⦘ ≡ jf S ⨾ (sb S ⨾ ⦗F S⦘)^? ⨾ ⦗Acq S⦘.
+Proof. 
+  arewrite (sb S ⨾ ⦗F S'⦘ ≡ sb S ⨾ ⦗F S⦘).
+  { rewrite ES.sbE; auto. rewrite !seqA.
+    arewrite (⦗E S⦘ ⨾ ⦗F S'⦘ ≡ ⦗E S⦘ ⨾ ⦗F S⦘); auto.
+    rewrite !seq_eqv.
+    apply eqv_rel_more.
+    eapply basic_step_f_eq_f; eauto. }
+  assert (jf S ⨾ (sb S ⨾ ⦗F S⦘)^? ≡
+          jf S ⨾ (sb S ⨾ ⦗F S⦘)^? ⨾ ⦗E S⦘) as HH.
+  { split; [|basic_solver 10].
+    rewrite (dom_r WF.(ES.jfE)).
+    rewrite (dom_r WF.(ES.sbE)).
+    basic_solver 20. }
+  seq_rewrite HH. symmetry.
+  seq_rewrite HH. rewrite !seqA.
+  rewrite <- !id_inter.
+  rewrite basic_step_acq_eq_acq with (S':=S'); eauto.
+Qed.
+
+(******************************************************************************)
+(** ** Deltas lemmas *)
+(******************************************************************************)
+
+Lemma add_jf_jf_delta_dom w e e' S S'
+      (BSTEP : basic_step e e' S S') 
+      (AJF : add_jf w e S S') 
+      (wf : ES.Wf S) : 
+  dom_rel (jf_delta w e) ⊆₁ E S.
+Proof. 
+  cdes AJF; cdes BSTEP; cdes BSTEP_.
+  step_solver.
+Qed.  
+
+Lemma add_jf_jf_deltaE w e e' S S'
+      (BSTEP : basic_step e e' S S') 
+      (AJF : add_jf w e S S') 
+      (wf : ES.Wf S) : 
+  jf_delta w e ⨾ ⦗E S⦘ ≡ ∅₂. 
+Proof. 
+  cdes AJF; cdes BSTEP; cdes BSTEP_.
+  split; [|done].
+  step_solver.
+Qed.  
+
+Lemma add_jf_jfi_delta_dom lang k k' st st' w e e' S S'
+      (BSTEP_ : basic_step_ lang k k' st st' e e' S S') 
+      (AJF : add_jf w e S S') 
+      (wf : ES.Wf S) : 
+  dom_rel (jfi_delta S k w e) ⊆₁ E S.
+Proof. 
+  cdes AJF; cdes BSTEP_.
+  step_solver.
+Qed.  
+
+Lemma add_jf_jfe_delta_dom lang k k' st st' w e e' S S'
+      (BSTEP_ : basic_step_ lang k k' st st' e e' S S') 
+      (AJF : add_jf w e S S') 
+      (wf : ES.Wf S) : 
+  dom_rel (jfe_delta S k w e) ⊆₁ E S.
+Proof. 
+  cdes AJF; cdes BSTEP_.
+  step_solver.
+Qed.
+
+Lemma add_jf_jfi_deltaE lang k k' st st' w e e' S S'
+      (BSTEP_ : basic_step_ lang k k' st st' e e' S S') 
+      (AJF : add_jf w e S S') 
+      (wf : ES.Wf S) : 
+  jfi_delta S k w e ⨾ ⦗E S⦘ ≡ ∅₂.
+Proof. 
+  cdes AJF; cdes BSTEP_.
+  split; [|done].
+  step_solver.
+Qed.  
+
+Lemma add_jf_jfe_deltaE lang k k' st st' w e e' S S'
+      (BSTEP_ : basic_step_ lang k k' st st' e e' S S') 
+      (AJF : add_jf w e S S') 
+      (wf : ES.Wf S) : 
+  jfe_delta S k w e ⨾ ⦗E S⦘ ≡ ∅₂.
+Proof. 
+  cdes AJF; cdes BSTEP_.
+  split; [|done].
+  step_solver.
+Qed.  
+
+Lemma basic_step_sw_delta_dom lang k k' st st' e e' S S'
+      (BSTEP_ : basic_step_ lang k k' st st' e e' S S') 
+      (wfE: ES.Wf S) :
+  dom_rel (sw_delta S S' k e e') ⊆₁ E S.
+Proof. 
+  cdes BSTEP_.
+  step_solver.
+Qed.
+
+Lemma basic_step_sw_deltaE lang k k' st st' e e' S S'
+      (BSTEP_ : basic_step_ lang k k' st st' e e' S S') 
+      (wfE: ES.Wf S) :
+  sw_delta S S' k e e' ⨾ ⦗E S⦘ ≡ ∅₂.
+Proof. 
+  cdes BSTEP_.
+  split; [|done]. 
+  unfold sw_delta.
+  step_solver.
+Qed.
+
+Lemma basic_step_hb_delta_dom lang k k' st st' e e' S S' 
+      (BSTEP_ : basic_step_ lang k k' st st' e e' S S') 
+      (wfE: ES.Wf S) :
+  dom_rel (hb_delta S S' k e e') ⊆₁ E S ∪₁ eq e.
+Proof. 
+  cdes BSTEP_.
+  unfold hb_delta.
+  rewrite crE, !seq_union_l, seq_id_l. 
+  rewrite !dom_union, !dom_seq.
+  rewrite !set_subset_union_l.
+  splits. 
+  { eapply basic_step_sb_delta_dom; eauto. }
+  all : step_solver.
+Qed. 
+
+Lemma basic_step_hb_deltaE lang k k' st st' e e' S S' 
+      (BSTEP_ : basic_step_ lang k k' st st' e e' S S') 
+      (wfE: ES.Wf S) :
+  hb_delta S S' k e e' ⨾ ⦗E S⦘ ≡ ∅₂.
+Proof. 
+  cdes BSTEP_.
+  split; [|done].
+  step_solver.
+Qed.
+
+Lemma basic_step_hb_delta_alt lang k k' st st' e e' S S'
+      (BSTEP_ : basic_step_ lang k k' st st' e e' S S') 
+      (wfE: ES.Wf S) :
+  hb_delta S S' k e e' ≡ 
+    (hb S)^? ⨾ ((sb_delta S k e e' ∪ sw_delta S S' k e e') ⨾ (hb S)^?)⁺.
+Proof. 
+  cdes BSTEP_.
+  unfold hb_delta. 
+  apply seq_more; auto.
+  rewrite !crE. relsf.
+  rewrite hbE; auto.
+  arewrite_false (sb_delta S k e e' ⨾ ⦗E S⦘).
+  { eapply basic_step_sb_deltaE; eauto. }
+  arewrite_false (sw_delta S S' k e e' ⨾ ⦗E S⦘).
+  { eapply basic_step_sw_deltaE; eauto. }
+  relsf.
+  rewrite ct_begin, rtE. relsf.
+  rewrite !unionA.
+  do 3 (apply union_more; auto).
+  { rewrite ct_begin, rtE. relsf.
+    rewrite <- !seqA.
+    arewrite_false (sb_delta S k e e' ⨾ sw_delta S S' k e e'). 
+    { step_solver. }
+    rewrite <- !seqA.
+    arewrite 
+      (sb_delta S k e e' ⨾ sb_delta S k e e' ≡ 
+                            sb_delta S k e e' ⨾ eq e × eq_opt e').
+    { rewrite dom_rel_helper with (r := sb_delta S k e e') at 2.
+      2 : eapply basic_step_sb_delta_dom; eauto.
+      rewrite id_union. relsf. 
+      arewrite_false (sb_delta S k e e' ⨾ ⦗E S⦘).
+      { step_solver. }
+      relsf.
+      apply seq_more; auto.
+      unfold sb_delta. 
+      rewrite cross_union_r. relsf.
+      arewrite_false (⦗eq e⦘ ⨾ ES.cont_sb_dom S k × eq e). 
+      { step_solver. }
+      arewrite_false (⦗eq e⦘ ⨾ ES.cont_sb_dom S k × eq_opt e'). 
+      { step_solver. }
+      basic_solver 20. }
+    relsf.
+    rewrite ct_begin, rtE. relsf.
+
+    arewrite_false (eq e × eq_opt e' ⨾ sb_delta S k e e').
+    { step_solver. }
+    arewrite_false (eq e × eq_opt e' ⨾ sb_delta S k e e').
+    { step_solver. }
+    arewrite_false (eq e × eq_opt e' ⨾ sw_delta S S' k e e').
+    { step_solver. }
+    arewrite_false (eq e × eq_opt e' ⨾ sw_delta S S' k e e').
+    { step_solver. }
+    basic_solver 10. }
+
+  rewrite ct_begin, rtE. relsf.
+  rewrite <- !seqA.
+  arewrite_false (sw_delta S S' k e e' ⨾ sw_delta S S' k e e'). 
+  { unfold sw_delta. step_solver. }
+  rewrite <- !seqA.
+  arewrite 
+    (sw_delta S S' k e e' ⨾ sb_delta S k e e' ≡ 
+              sw_delta S S' k e e' ⨾ eq e × eq_opt e').
+  { rewrite dom_rel_helper with (r := sb_delta S k e e').
+    2 : eapply basic_step_sb_delta_dom; eauto.
+    rewrite id_union. relsf. 
+    arewrite_false (sw_delta S S' k e e' ⨾ ⦗E S⦘).
+    { unfold sw_delta. step_solver. }
+    unfold sb_delta. 
+    rewrite cross_union_r. relsf.
+    arewrite_false (⦗eq e⦘ ⨾ ES.cont_sb_dom S k × eq e).
+    { step_solver. }
+    arewrite_false (⦗eq e⦘ ⨾ ES.cont_sb_dom S k × eq_opt e').
+    { step_solver. }
+    basic_solver 10. }
+  
+  relsf.
+  rewrite ct_begin, rtE. relsf.
+  arewrite_false (eq e × eq_opt e' ⨾ sb_delta S k e e').
+  { step_solver. }
+  arewrite_false (eq e × eq_opt e' ⨾ sb_delta S k e e').
+  { step_solver. }
+  arewrite_false (eq e × eq_opt e' ⨾ sw_delta S S' k e e').
+  { step_solver. }
+  arewrite_false (eq e × eq_opt e' ⨾ sw_delta S S' k e e').
+  { step_solver. }
+  basic_solver 10.   
+Qed.
+
+(******************************************************************************)
+(** ** add_jf properties *)
+(******************************************************************************)
+
+Lemma add_jf_jf_dom w e e' S S'
+      (BSTEP : basic_step e e' S S')
+      (AJF : add_jf w e S S') 
+      (wf : ES.Wf S) : 
+  dom_rel (jf S') ⊆₁ E S.
+Proof. 
+  cdes AJF; cdes BSTEP; cdes BSTEP_.
+  rewrite JF', dom_union. 
+  rewrite wf.(ES.jfE).
+  rewrite add_jf_jf_delta_dom; eauto.
+  basic_solver.
+Qed.
+
+Lemma add_jf_jfE w e e' S S'
+      (BSTEP : basic_step e e' S S') 
+      (AJF : add_jf w e S S') 
+      (wf : ES.Wf S) : 
+  jf S' ⨾ ⦗E S⦘ ≡ jf S.
+Proof.   
+  cdes AJF; cdes BSTEP; cdes BSTEP_.
+  rewrite JF'. 
+  rewrite seq_union_l.
+  rewrite add_jf_jf_deltaE; eauto.
+  rewrite ES.jfE; auto. basic_solver 5.
+Qed.
+
+Lemma add_jf_jfi lang k k' st st' w e e' S S'
+      (BSTEP_ : basic_step_ lang k k' st st' e e' S S') 
+      (AJF : add_jf w e S S') 
+      (wf : ES.Wf S) : 
+  jfi S' ≡ jfi S ∪ jfi_delta S k w e.
+Proof. 
+  cdes AJF; cdes BSTEP_.
+  unfold ES.jfi, jfi_delta.
+  rewrite SB', JF'.
+  rewrite inter_union_l, !inter_union_r.
+  arewrite_false (jf S ∩ sb_delta S k e e').
+  { step_solver. }
+  arewrite_false (jf_delta w e ∩ sb S). 
+  { step_solver. } 
+  relsf.
+  apply union_more; auto.
+  autounfold with ESStepDb.
+  rewrite inter_union_r.
+  arewrite_false (singl_rel w e ∩ (ES.cont_sb_dom S k ∪₁ eq e) × eq_opt e').
+  { step_solver. }
+  basic_solver 10.
+Qed.
+
+Lemma add_jf_jfe lang k k' st st' w e e' S S'
+      (BSTEP_ : basic_step_ lang k k' st st' e e' S S') 
+      (AJF : add_jf w e S S') 
+      (wf : ES.Wf S) : 
+  jfe S' ≡ jfe S ∪ jfe_delta S k w e.
+Proof. 
+  cdes AJF; cdes BSTEP_.
+  unfold ES.jfe, jfe_delta.
+  rewrite SB', JF'.
+  rewrite minus_union_l, !minus_union_r.
+  erewrite minus_disjoint 
+    with (r := jf S) (r' := sb_delta S k e e').
+  2 : { split; [|done]. step_solver. }
+  erewrite minus_disjoint 
+    with (r := jf_delta w e) (r' := sb S).
+  2 : { split; [|done]. step_solver. }
+  apply union_more.
+  { basic_solver. }
+  autounfold with ESStepDb.
+  rewrite !minus_union_r.
+  erewrite minus_disjoint 
+    with (r := singl_rel w e) (r' := (ES.cont_sb_dom S k ∪₁ eq e) × eq_opt e').
+  2 : { split; [|done]. step_solver. }
+  rewrite minus_inter_compl.
+  rewrite !interC with (r1 := singl_rel w e).
+  rewrite !interA, !interK.
+  split; [basic_solver|].
+  unfolder. ins. desc.
+  splits; auto. 
+  red. ins. desc. auto.
+Qed.
+
+Lemma add_jf_jfi_dom w e e' S S'
+      (BSTEP : basic_step e e' S S')
+      (AJF : add_jf w e S S') 
+      (wf : ES.Wf S) : 
+  dom_rel (jfi S') ⊆₁ E S.
+Proof. 
+  unfold ES.jfi.
+  unfolder; ins; desf.
+  eapply add_jf_jf_dom; eauto. 
+  basic_solver.
+Qed.
+
+Lemma add_jf_jfe_dom w e e' S S'
+      (BSTEP : basic_step e e' S S')
+      (AJF : add_jf w e S S') 
+      (wf : ES.Wf S) : 
+  dom_rel (jfe S') ⊆₁ E S.
+Proof. 
+  unfold ES.jfe.
+  unfolder; ins; desf.
+  eapply add_jf_jf_dom; eauto. 
+  basic_solver.
+Qed.
+
+Lemma add_jf_jfiE w e e' S S'
+      (BSTEP : basic_step e e' S S') 
+      (AJF : add_jf w e S S') 
+      (wf : ES.Wf S) : 
+  jfi S' ⨾ ⦗E S⦘ ≡ jfi S.
+Proof.   
+  cdes AJF; cdes BSTEP; cdes BSTEP_.
+  rewrite add_jf_jfi; eauto.
+  rewrite seq_union_l.
+  rewrite add_jf_jfi_deltaE; eauto.
+  rewrite ES.jfiE; auto. basic_solver 5.
+Qed.
+
+Lemma add_jf_jfeE w e e' S S'
+      (BSTEP : basic_step e e' S S') 
+      (AJF : add_jf w e S S') 
+      (wf : ES.Wf S) : 
+  jfe S' ⨾ ⦗E S⦘ ≡ jfe S.
+Proof.   
+  cdes AJF; cdes BSTEP; cdes BSTEP_.
+  rewrite add_jf_jfe; eauto.
+  rewrite seq_union_l.
+  rewrite add_jf_jfe_deltaE; eauto.
+  rewrite ES.jfeE; auto. basic_solver 5.
+Qed.
+
+Lemma add_jf_sb_jf lang k k' st st' w e e' S S'
+      (BSTEP_ : basic_step_ lang k k' st st' e e' S S') 
+      (AJF : add_jf w e S S') 
+      (wfE: ES.Wf S) :
+  (sb S' ∪ jf S')＊ ≡ 
+    (sb S ∪ jf S)＊ ⨾ 
+      (sb_delta S k e e' ∪ singl_rel w e ∪ eq w × eq_opt e')^?. 
+Proof. 
+  cdes AJF; cdes BSTEP_.
+  assert (basic_step e e' S S') as BSTEP.
+  { econstructor. eauto. }
+  autounfold with ESStepDb in *.
+  rewrite SB', JF'. 
+  arewrite 
+    (sb S ∪ sb_delta S k e e' ∪ (jf S ∪ singl_rel w e) ≡
+      sb_delta S k e e' ∪ singl_rel w e ∪ (sb S ∪ jf S))
+    by basic_solver.
+  erewrite rt_unionE. 
+  apply seq_more; auto.
+  rewrite rt_begin with (r := sb S ∪ jf S).
+  rewrite seq_union_r, seq_id_r. 
+  arewrite_false 
+    ((sb_delta S k e e' ∪ singl_rel w e) ⨾ (sb S ∪ jf S)).
+  { step_solver. }
+  relsf. 
+  rewrite rtE, crE.
+  apply union_more; auto.
+  (* unroll transitive closure up to 3 iterations *)
+  do 3 rewrite ct_begin, rtE.
+  rewrite !seq_union_r, !seq_id_r.
+  rewrite <- !seqA.
+  arewrite 
+    ((sb_delta S k e e' ∪ singl_rel w e)
+     ⨾ (sb_delta S k e e' ∪ singl_rel w e) ≡ 
+     ES.cont_sb_dom S k × eq_opt e' ∪ eq w × eq_opt e'). 
+  { unfold sb_delta.
+    rewrite !seq_union_l. 
+    arewrite_false 
+      ((ES.cont_sb_dom S k ∪₁ eq e) × eq_opt e'
+      ⨾ (ES.cont_sb_dom S k × eq e ∪ 
+                        (ES.cont_sb_dom S k ∪₁ eq e) × eq_opt e' ∪ singl_rel w e)). 
+    { arewrite (singl_rel w e ⊆ E S × eq e).
+      { basic_solver. }
+      step_solver. }
+    rewrite cross_union_r. rewrite !seq_union_r.
+    arewrite_false 
+      (ES.cont_sb_dom S k × eq e ⨾ ES.cont_sb_dom S k × eq_opt e').
+    { step_solver. }
+    arewrite_false
+     (ES.cont_sb_dom S k × eq e ⨾ singl_rel w e).
+    { arewrite (singl_rel w e ⊆ E S × eq e).
+      { basic_solver. }
+      step_solver. }
+    arewrite_false
+      (singl_rel w e ⨾ ES.cont_sb_dom S k × eq e).
+    { step_solver. }
+    arewrite_false
+      (singl_rel w e ⨾ ES.cont_sb_dom S k × eq_opt e').
+    { step_solver. }
+    arewrite_false
+      (ES.cont_sb_dom S k × eq e ⨾ ES.cont_sb_dom S k × eq e).
+    { step_solver. }
+    arewrite_false
+      (singl_rel w e ⨾ singl_rel w e).
+    { arewrite (singl_rel w e ⊆ E S × eq e).
+      { basic_solver. }
+      step_solver. }
+    basic_solver 10. }
+  rewrite <- seqA.
+  arewrite_false 
+    ((ES.cont_sb_dom S k × eq_opt e' ∪ eq w × eq_opt e')
+        ⨾ (sb_delta S k e e' ∪ singl_rel w e)).
+  { arewrite (singl_rel w e ⊆ E S × eq e).
+    { basic_solver. }
+    step_solver. }
+  unfold sb_delta. 
+  basic_solver 10. 
+Qed.
+
+Lemma add_jf_sb_jfE w e e' S S'
+      (BSTEP : basic_step e e' S S') 
+      (AJF : add_jf w e S S') 
+      (wfE: ES.Wf S) :
+  (sb S' ∪ jf S')＊ ⨾ ⦗E S⦘ ≡ (sb S ∪ jf S)＊ ⨾ ⦗E S⦘.
+Proof. 
+  cdes AJF; cdes BSTEP; cdes BSTEP_.
+  erewrite add_jf_sb_jf; eauto.
+  rewrite crE. relsf.
+  rewrite <- union_false_r with (r := (sb S ∪ jf S)＊ ⨾ ⦗E S⦘) at 2. 
+  apply union_more; auto.
+  split; [|done].
+  step_solver.
+Qed.
+
+Lemma add_jf_sb_jf_dom w e e' S S'
+      (BSTEP : basic_step e e' S S') 
+      (AJF : add_jf w e S S') 
+      (wfE: ES.Wf S) :
+  dom_rel ((sb S' ∪ jf S')＊ ⨾ ⦗E S⦘) ⊆₁ E S.
+Proof. 
+  rewrite add_jf_sb_jfE; eauto.
+  rewrite rtE, seq_union_l, seq_id_l. 
+  rewrite ES.sbE, ES.jfE; auto.
+  rewrite <- seq_union_r. 
+  rewrite inclusion_ct_seq_eqv_l.
+  basic_solver.
+Qed.
+
+Lemma add_jf_cc lang k k' st st' w e e' S S'
+      (BSTEP_ : basic_step_ lang k k' st st' e e' S S') 
+      (AJF : add_jf w e S S') 
+      (wfE: ES.Wf S) :
+  cc S' ≡ cc S ∪ 
+     cf S' ∩ 
+     (jfe S ⨾ (sb S ∪ jf S)＊ ⨾ 
+          (jfe S ⨾ sb_delta S k e e' ∪ jfe_delta S k w e ⨾ (eq e × eq_opt e')^?)).
+Proof. 
+  cdes AJF; cdes BSTEP_.
+  assert (basic_step e e' S S') as BSTEP.
+  { econstructor. eauto. }
+  unfold cc at 1. 
+  erewrite dom_rel_helper with (r := jfe S') at 2.
+  2 : eapply add_jf_jfe_dom; eauto.
+  rewrite !seqA. 
+  rewrite <- seqA with (r2 := ⦗E S⦘).
+  erewrite dom_rel_helper with (r := (sb S' ∪ jf S')＊ ⨾ ⦗E S⦘).
+  2 : eapply add_jf_sb_jf_dom; eauto.
+  rewrite add_jf_sb_jfE; eauto.
+  rewrite !seqA. 
+  rewrite <- !seqA with (r2 := ⦗E S⦘).
+  rewrite add_jf_jfeE; eauto.
+  rewrite !seqA.
+  rewrite <- !seqA with (r1 := ⦗E S⦘).
+  erewrite <- dom_rel_helper with (r := jfe S').
+  2 : eapply add_jf_jfe_dom; eauto.  
+  rewrite SB'. 
+  rewrite add_jf_jfe with (S' := S') at 1; eauto.
+  rewrite cr_union_l. relsf.
+  rewrite !inter_union_r.
+  rewrite unionA.
+  apply union_more.
+  { rewrite basic_step_cf; eauto. 
+    autounfold with ESStepDb.
+    rewrite <- unionA, !inter_union_l, unionA.
+    rewrite <- union_false_r with (r := cc S).
+    apply union_more.
+    { by unfold cc. }
+    split; [|done].
+    step_solver. }
+  rewrite unionC, unionA.
+  apply union_more; auto.
+  rewrite !crE. relsf.
+  arewrite_false (jfe_delta S k w e ⨾ sb S). 
+  { autounfold with ESStepDb. 
+    arewrite (singl_rel w e ⊆ E S × eq e).
+    { basic_solver. }
+    step_solver. }
+  relsf.
+  rewrite !inter_union_r.
+  rewrite unionC.
+  apply union_more; auto.
+  apply inter_rel_more; auto.  
+  do 2 (apply seq_more; auto).  
+  autounfold with ESStepDb. 
+  rewrite cross_union_r.
+  relsf. rewrite !seqA.
+  arewrite_false (singl_rel w e ⨾ ES.cont_sb_dom S k × eq e).
+  { arewrite (singl_rel w e ⊆ E S × eq e).
+    { basic_solver. }
+    step_solver. }
+  arewrite_false (singl_rel w e ⨾ ES.cont_sb_dom S k × eq_opt e').
+  { arewrite (singl_rel w e ⊆ E S × eq e).
+    { basic_solver. }
+    step_solver. }
+  basic_solver 10.
+Qed.  
+
+Lemma add_jf_ccE w e e' S S'
+      (BSTEP : basic_step e e' S S') 
+      (AJF : add_jf w e S S') 
+      (wfE: ES.Wf S) :
+  cc S' ⨾ ⦗E S⦘ ≡ cc S.
+Proof. 
+  cdes AJF; cdes BSTEP; cdes BSTEP_.
+  rewrite add_jf_cc; eauto.
+  rewrite seq_union_l.
+  rewrite interC.
+  rewrite <- lib.AuxRel.seq_eqv_inter_lr.
+  rewrite !seqA, seq_union_l.
+  rewrite !seqA.
+  arewrite_false 
+    (sb_delta S k e e' ⨾ ⦗E S⦘).
+  { step_solver. }
+  arewrite_false
+   (jfe_delta S k w e ⨾ (eq e × eq_opt e')^? ⨾ ⦗E S⦘).
+  { autounfold with ESStepDb. 
+    arewrite (singl_rel w e ⊆ E S × eq e).
+    { basic_solver. }
+    step_solver. }
+  relsf.
+  rewrite ccE. basic_solver.
+Qed.
+
+Lemma add_jf_jf_rmw w e e' S S'
+      (BSTEP : basic_step e e' S S') 
+      (AJF : add_jf w e S S') 
+      (wfE: ES.Wf S) :
+  jf S' ⨾ rmw S' ≡ jf S ⨾ rmw S ∪ eq w × eq_opt e'.
+Proof. 
+  cdes AJF; cdes BSTEP; cdes BSTEP_.
+  rewrite JF', RMW'.
+  relsf. rewrite unionA.
+  apply union_more; auto.
+  arewrite_false (jf_delta w e ⨾ rmw S).
+  { step_solver. }
+  arewrite_false (jf S ⨾ rmw_delta e e').
+  { step_solver. }
+  autounfold with ESStepDb.
+  basic_solver 10.
+Qed.  
+
+Lemma add_jf_jf_rmwE w e e' S S'
+      (BSTEP : basic_step e e' S S') 
+      (AJF : add_jf w e S S') 
+      (wfE: ES.Wf S) :
+  jf S' ⨾ rmw S' ⨾ ⦗E S⦘ ≡ jf S ⨾ rmw S.
+Proof. 
+  cdes AJF; cdes BSTEP; cdes BSTEP_.
+  rewrite <- seqA.
+  rewrite add_jf_jf_rmw; eauto.
+  relsf.
+  arewrite_false (eq w × eq_opt e' ⨾ ⦗E S⦘).
+  { step_solver. }
+  rewrite ES.rmwE; auto. basic_solver 10.
+Qed.
+
+Lemma add_jf_rsE w e e' S S'
+      (BSTEP : basic_step e e' S S') 
+      (AJF : add_jf w e S S') 
+      (wfE: ES.Wf S) :
+  rs S' ⨾ ⦗E S⦘ ≡ rs S ⨾ ⦗E S⦘.
+Proof. 
+  cdes AJF; cdes BSTEP; cdes BSTEP_.
+  unfold rs at 1. rewrite !seqA.
+  arewrite ((jf S' ⨾ rmw S')＊ ⨾ ⦗E S⦘ ≡ (jf S ⨾ rmw S)＊ ⨾ ⦗E S⦘).
+  { rewrite !rtE. relsf.
+    eapply union_more; auto.
+    split. 
+    { rewrite !seq_eqv_r.
+      intros x y [TC Ey].
+      split; auto.
+      induction TC. 
+      { eapply t_step.
+        eapply add_jf_jf_rmwE; eauto.
+        unfolder in *. desc. eauto. }
+      eapply t_trans; eauto.
+      eapply IHTC1.
+      eapply add_jf_jf_dom; eauto.
+      apply ct_begin in TC2.
+      generalize TC2. basic_solver 10. }
+    apply seq_mori; [|done].
+    apply clos_trans_mori. 
+    rewrite add_jf_jf_rmw with (S' := S'); eauto.
+    basic_solver. }
+  arewrite ((jf S ⨾ rmw S)＊ ⨾ ⦗E S⦘ ≡ ⦗E S⦘ ⨾ (jf S ⨾ rmw S)＊ ⨾ ⦗E S⦘).
+  { rewrite rtE. relsf.
+    apply union_more; auto.
+    rewrite restr_clos_trans_eq with (s := E S).
+    2 : { rewrite ES.jfE, ES.rmwE; auto. basic_solver 10. }
+    basic_solver. }
+  seq_rewrite basic_step_w_sb_loc_wE; eauto.
+  unfold rs.
+  rewrite !seqA.
+  basic_solver.
+Qed.
+
+Lemma add_jf_releaseE w e e' S S'
+      (BSTEP : basic_step e e' S S') 
+      (AJF : add_jf w e S S') 
+      (wfE: ES.Wf S) :
+  release S' ⨾ ⦗E S⦘ ≡ release S ⨾ ⦗E S⦘.
+Proof. 
+  unfold release at 1.
+  rewrite !seqA.
+  arewrite (rs S' ⨾ ⦗E S⦘ ≡ ⦗E S⦘ ⨾ rs S ⨾ ⦗E S⦘).
+  { rewrite add_jf_rsE; eauto.
+    rewrite rsE; auto.
+    basic_solver. }
+  seq_rewrite basic_step_rel_f_sbE; eauto. 
+  unfold release.
+  rewrite ES.sbE, rsE; auto.
+  basic_solver 20.
+Qed.
+
+Lemma add_jf_sw lang k k' st st' w e e' S S'
+      (BSTEP_ : basic_step_ lang k k' st st' e e' S S') 
+      (AJF : add_jf w e S S') 
+      (nF' : eq_opt e' ∩₁ F S' ⊆₁ ∅)
+      (wfE: ES.Wf S) :
+  sw S' ≡ sw S ∪ sw_delta S S' k e e'. 
+Proof. 
+  cdes AJF; cdes BSTEP_.
+  assert (basic_step e e' S S') as BSTEP.
+  { econstructor. eauto. }
+  unfold sw_delta.
+  unfold sw at 1.
+  erewrite dom_rel_helper with (r := jf S').
+  2 : eapply add_jf_jf_dom; eauto.
+  rewrite !seqA, <- seqA.
+  rewrite add_jf_releaseE; eauto.
+  rewrite !seqA.
+  rewrite <- seqA with (r1 := ⦗E S⦘).
+  erewrite <- dom_rel_helper with (r := jf S').
+  2 : eapply add_jf_jf_dom; eauto.
+  rewrite SB', JF'.
+  rewrite seq_union_l, cr_union_l.
+  relsf. rewrite unionA.
+  apply union_more.
+  { rewrite basic_step_jf_sb_f_acq; eauto. }
+  rewrite crE. relsf.
+  rewrite !seqA.
+  arewrite_false (sb_delta S k e e' ⨾ ⦗F S'⦘).
+  { unfold sb_delta.
+    clear -nF' rR'.
+    rewrite seq_union_l, <- !cross_inter_r.
+    arewrite (eq e ∩₁ F S' ⊆₁ ∅).
+    { type_solver. }
+    rewrite nF'.
+    basic_solver. }
+  arewrite_false (jf_delta w e ⨾ sb S).
+  { step_solver. }
+  arewrite_false (jf S ⨾ ⦗eq e⦘).
+  { step_solver. }
+  unfold jf_delta.
+  basic_solver 10.
+Qed.  
+
+Lemma add_jf_sw_dom lang k k' st st' w e e' S S'
+      (BSTEP_ : basic_step_ lang k k' st st' e e' S S') 
+      (AJF : add_jf w e S S') 
+      (nF' : eq_opt e' ∩₁ F S' ⊆₁ ∅)
+      (wfE: ES.Wf S) :
+  dom_rel (sw S') ⊆₁ E S.
+Proof. 
+  cdes AJF; cdes BSTEP_.
+  rewrite add_jf_sw; eauto.
+  step_solver.
+Qed.
+
+Lemma add_jf_swE w e e' S S' 
+      (BSTEP : basic_step e e' S S') 
+      (AJF : add_jf w e S S') 
+      (nF' : eq_opt e' ∩₁ F S' ⊆₁ ∅)
+      (wfE: ES.Wf S) :
+  sw S' ⨾ ⦗E S⦘ ≡ sw S.
+Proof. 
+  cdes AJF; cdes BSTEP; cdes BSTEP_.
+  rewrite add_jf_sw; eauto.
+  relsf. rewrite basic_step_sw_deltaE; eauto.
+  rewrite swE; auto. basic_solver 5.
+Qed.
+
+Lemma add_jf_hb lang k k' st st' w e e' S S' 
+      (BSTEP_ : basic_step_ lang k k' st st' e e' S S') 
+      (AJF : add_jf w e S S') 
+      (nF' : eq_opt e' ∩₁ F S' ⊆₁ ∅)
+      (wfE: ES.Wf S) :
+  hb S' ≡ hb S ∪ hb_delta S S' k e e'.
+Proof.
+  cdes AJF; cdes BSTEP_.
+  assert (basic_step e e' S S') as BSTEP.
+  { subst. econstructor. eauto. }
+  unfold hb at 1.
+  rewrite SB'. 
+  rewrite add_jf_sw; eauto.
+  arewrite 
+    (sb S ∪ sb_delta S k e e' ∪ (sw S ∪ sw_delta S S' k e e') ≡
+     (sb_delta S k e e' ∪ sw_delta S S' k e e') ∪ (sb S ∪ sw S))
+    by basic_solver.
+  rewrite ct_unionE.
+  unfold hb. 
+  apply union_more; auto.
+  rewrite <- cr_of_ct.
+  rewrite basic_step_hb_delta_alt; eauto.
+Qed.
+
+Lemma add_jf_hb_dom w e e' S S' 
+      (BSTEP : basic_step e e' S S') 
+      (AJF : add_jf w e S S') 
+      (nF' : eq_opt e' ∩₁ F S' ⊆₁ ∅)
+      (wfE: ES.Wf S) :
+  dom_rel (hb S') ⊆₁ E S ∪₁ eq e.
+Proof. 
+  cdes AJF; cdes BSTEP; cdes BSTEP_.
+  rewrite add_jf_hb; eauto.
+  rewrite dom_union.
+  rewrite basic_step_hb_delta_dom; eauto.
+  rewrite hbE; auto.
+  basic_solver.
+Qed. 
+
+Lemma add_jf_hbE w e e' S S' 
+      (BSTEP : basic_step e e' S S') 
+      (AJF : add_jf w e S S') 
+      (nF' : eq_opt e' ∩₁ F S' ⊆₁ ∅)
+      (wfE: ES.Wf S) :
+  hb S' ⨾ ⦗E S⦘ ≡ hb S.
+Proof. 
+  cdes AJF; cdes BSTEP; cdes BSTEP_.
+  rewrite add_jf_hb; eauto.
+  relsf.
+  rewrite basic_step_hb_deltaE; eauto.
+  rewrite hbE; auto. basic_solver 5.
+Qed. 
